books/centaur/fgl/bvar-db-equivs.lisp
@@ -149,6 +149,7 @@
                               state)
   :guard (and (<= (base-bvar bvar-db) bvar)
               (< bvar (next-bvar bvar-db)))
+  :returns (new-bvar-db)
   (declare (ignorable state))
   (gl-object-case test-obj
     :g-var (add-term-equiv test-obj bvar bvar-db)
@@ -172,4 +173,75 @@
                bvar-db)
 
     :otherwise bvar-db))
+
+
+
+(define bvar-db-bfrlist-aux ((n natp) bvar-db)
+  :returns (bfrs)
+  :measure (nfix (- (nfix n) (base-bvar bvar-db)))
+  :guard (and (<= (base-bvar bvar-db) n)
+              (<= n (next-bvar bvar-db)))
+  (if (zp (- (lnfix n) (base-bvar bvar-db)))
+      nil
+    (append (gl-object-bfrlist (get-bvar->term (1- (lnfix n)) bvar-db))
+            (bvar-db-bfrlist-aux (1- (lnfix n)) bvar-db)))
+  ///
+  (defthm bfrlist-aux-of-get-bvar->term
+    (implies (and (not (member v (bvar-db-bfrlist-aux n bvar-db)))
+                  (< (nfix m) (nfix n))
+                  (<= (base-bvar$a bvar-db) (nfix m)))
+             (not (member v (gl-object-bfrlist (get-bvar->term$a m bvar-db))))))
+
+  (defthm bfrlist-aux-of-add-term-bvar
+    (implies (<= (nfix n) (next-bvar$a bvar-db))
+             (equal (bvar-db-bfrlist-aux n (add-term-bvar$a obj bvar-db))
+                    (bvar-db-bfrlist-aux n bvar-db))))
+
+  (defthm bfrlist-aux-of-update-term-equivs
+    (equal (bvar-db-bfrlist-aux n (update-term-equivs$a obj bvar-db))
+           (bvar-db-bfrlist-aux n bvar-db)))
+
+  (defthm subsetp-bfrlist-of-bvar-db-bfrlist-aux
+    (implies (and (< (nfix m) (nfix n))
+                  (<= (base-bvar$a bvar-db) (nfix m)))
+             (subsetp (gl-object-bfrlist (get-bvar->term$a m bvar-db))
+                      (bvar-db-bfrlist-aux n bvar-db)))
+    :hints(("Goal" :in-theory (enable acl2::subsetp-witness-rw)))))
+
+(define bvar-db-bfrlist (bvar-db)
+  (bvar-db-bfrlist-aux (next-bvar bvar-db) bvar-db)
+  ///
+  (defthm bfrlist-of-get-bvar->term
+    (implies (and (not (member v (bvar-db-bfrlist bvar-db)))
+                  (< (nfix m) (next-bvar$a bvar-db))
+                  (<= (base-bvar$a bvar-db) (nfix m)))
+             (not (member v (gl-object-bfrlist (get-bvar->term$a m bvar-db))))))
+
+  (defthm bvar-db-bfrlist-of-add-term-bvar
+    (equal (bvar-db-bfrlist (add-term-bvar$a obj bvar-db))
+           (append (gl-object-bfrlist obj)
+                   (bvar-db-bfrlist bvar-db)))
+    :hints (("goal" :in-theory (enable bvar-db-bfrlist-aux))))
+
+  (defthm subsetp-bfrlist-of-bvar-db-bfrlist
+    (implies (and (< (nfix m) (next-bvar$a bvar-db))
+                  (<= (base-bvar$a bvar-db) (nfix m)))
+             (subsetp (gl-object-bfrlist (get-bvar->term$a m bvar-db))
+                      (bvar-db-bfrlist bvar-db))))
+
+  (defthm bvar-db-bfrlist-of-add-term-bvar-unique
+    (acl2::set-equiv (bvar-db-bfrlist (mv-nth 1 (add-term-bvar-unique obj bvar-db)))
+                     (append (gl-object-bfrlist obj)
+                             (bvar-db-bfrlist bvar-db)))
+    :hints (("goal" :in-theory (e/d (add-term-bvar-unique)
+                                    (bvar-db-bfrlist
+                                     subsetp-bfrlist-of-bvar-db-bfrlist))
+             :use ((:instance subsetp-bfrlist-of-bvar-db-bfrlist
+                    (m (get-term->bvar$a obj bvar-db)))))))
+
+  (defthm bvar-db-bfrlist-of-maybe-add-equiv-term
+    (equal (bvar-db-bfrlist (maybe-add-equiv-term obj bvar bvar-db state))
+           (bvar-db-bfrlist bvar-db))
+    :hints(("Goal" :in-theory (enable maybe-add-equiv-term
+                                      add-term-equiv)))))
 
