books/centaur/fgl/interp.lisp
@@ -36,6 +36,128 @@
 (include-book "glcp-unify-defs")
 (include-book "centaur/meta/bindinglist" :dir :system)
 (include-book "syntax-bind")
+(include-book "rewrite-tables")
+(include-book "system/f-put-global" :dir :system)
+(include-book "std/util/defret-mutual-generate" :dir :system)
+
+
+
+(define interp-st-bfrs-ok (interp-st)
+  (b* ((constraint-db (interp-st->constraint-db interp-st))
+       (constraint-insts (interp-st->constraint-inst-stack interp-st))
+       (thenvals (interp-st->thenval-stack interp-st))
+       (elsevals (interp-st->elseval-stack interp-st)))
+    (stobj-let ((logicman (interp-st->logicman interp-st))
+                (bvar-db (interp-st->bvar-db interp-st))
+                (stack (interp-st->stack interp-st))
+                (pathcond (interp-st->pathcond interp-st))
+                (constraint-pathcond (interp-st->constraint interp-st)))
+               (ok)
+               (b* ((bfrstate (logicman->bfrstate)))
+                 (and (bfr-listp (major-stack-bfrlist (stack-extract stack)))
+                      (bfr-listp (constraint-db-bfrlist constraint-db))
+                      (bfr-listp (constraint-instancelist-bfrlist constraint-insts))
+                      (bfr-listp (gl-objectlist-bfrlist thenvals))
+                      (bfr-listp (gl-objectlist-bfrlist elsevals))
+                      (ec-call (logicman-pathcond-p-fn pathcond logicman))
+                      (ec-call (logicman-pathcond-p-fn constraint-pathcond logicman))
+                      (not (bvar-db-bfrlist bvar-db))))
+               ok))
+  ///
+  (defthm interp-st-bfrs-ok-implies
+    (implies (interp-st-bfrs-ok interp-st)
+             (let* ((logicman (interp-st->logicman interp-st))
+                    (bfrstate (logicman->bfrstate)))
+               (and (bfr-listp (major-stack-bfrlist (interp-st->stack interp-st)))
+                    (bfr-listp (constraint-db-bfrlist (interp-st->constraint-db interp-st)))
+                    (logicman-pathcond-p (interp-st->pathcond interp-st))
+                    (logicman-pathcond-p (interp-st->constraint interp-st))
+                    (not (bvar-db-bfrlist (interp-st->bvar-db interp-st)))
+                    (bfr-listp (gl-objectlist-bfrlist (interp-st->thenval-stack interp-st)))
+                    (bfr-listp (gl-objectlist-bfrlist (interp-st->elseval-stack interp-st)))
+                    (implies (gl-objectlist-p (interp-st->thenval-stack interp-st))
+                             (gl-bfr-objectlist-p (interp-st->thenval-stack interp-st)))
+                    (implies (gl-objectlist-p (interp-st->elseval-stack interp-st))
+                             (gl-bfr-objectlist-p (interp-st->elseval-stack interp-st)))
+                    (bfr-listp (constraint-instancelist-bfrlist (interp-st->constraint-inst-stack interp-st)))))))
+
+  (acl2::def-updater-independence-thm interp-st-bfrs-ok-updater-independence
+    (implies (and (equal (interp-st-get :logicman new)
+                         (interp-st-get :logicman old))
+                  (equal (interp-st-get :stack new)
+                         (interp-st-get :stack old))
+                  (equal (interp-st-get :constraint-db new)
+                         (interp-st-get :constraint-db old))
+                  (equal (interp-st-get :pathcond new)
+                         (interp-st-get :pathcond old))
+                  (equal (interp-st-get :constraint new)
+                         (interp-st-get :constraint old))
+                  (equal (interp-st-get :bvar-db new)
+                         (interp-st-get :bvar-db old))
+                  (equal (interp-st-get :constraint new)
+                         (interp-st-get :constraint old))
+                  (equal (interp-st-get :constraint-inst-stack new)
+                         (interp-st-get :constraint-inst-stack old))
+                  (equal (interp-st-get :thenval-stack new)
+                         (interp-st-get :thenval-stack old))
+                  (equal (interp-st-get :elseval-stack new)
+                         (interp-st-get :elseval-stack old)))
+             (equal (interp-st-bfrs-ok new)
+                    (interp-st-bfrs-ok old))))
+
+
+  (defthm interp-st-bfrs-ok-of-logicman-extension
+    (implies (and (interp-st-bfrs-ok interp-st)
+                  (logicman-extension-p new-logicman (interp-st->logicman interp-st)))
+             (interp-st-bfrs-ok (update-interp-st->logicman new-logicman interp-st))))
+
+  (defthm interp-st-bfrs-ok-of-update-stack
+    (implies (And (interp-st-bfrs-ok interp-st)
+                  (bfr-listp (major-stack-bfrlist new-stack) (logicman->bfrstate (interp-st->logicman interp-st))))
+             (interp-st-bfrs-ok (update-interp-st->stack new-stack interp-st))))
+
+  (defthm interp-st-bfrs-ok-of-update-constraint-db
+    (implies (And (interp-st-bfrs-ok interp-st)
+                  (bfr-listp (constraint-db-bfrlist new-constraint-db) (logicman->bfrstate (interp-st->logicman interp-st))))
+             (interp-st-bfrs-ok (update-interp-st->constraint-db new-constraint-db interp-st))))
+
+  (defthm interp-st-bfrs-ok-of-update-pathcond
+    (implies (And (interp-st-bfrs-ok interp-st)
+                  (logicman-pathcond-p-fn new-pathcond (interp-st->logicman interp-st)))
+             (interp-st-bfrs-ok (update-interp-st->pathcond new-pathcond interp-st))))
+
+  (defthm interp-st-bfrs-ok-of-update-constraint
+    (implies (And (interp-st-bfrs-ok interp-st)
+                  (logicman-pathcond-p-fn new-constraint (interp-st->logicman interp-st)))
+             (interp-st-bfrs-ok (update-interp-st->pathcond new-constraint interp-st))))
+
+  (defthm interp-st-bfrs-ok-of-update-bvar-db
+    (implies (And (interp-st-bfrs-ok interp-st)
+                  (not (bvar-db-bfrlist new-bvar-db)))
+             (interp-st-bfrs-ok (update-interp-st->bvar-db new-bvar-db interp-st))))
+
+  (defthm interp-st-bfrs-ok-of-update-constraint-inst-stack
+    (implies (And (interp-st-bfrs-ok interp-st)
+                  (bfr-listp (constraint-instancelist-bfrlist new-constraint-stack)
+                             (logicman->bfrstate (interp-st->logicman interp-st))))
+             (interp-st-bfrs-ok (update-interp-st->constraint-inst-stack new-constraint-stack interp-st))))
+
+  (defthm interp-st-bfrs-ok-of-update-thenval-stack
+    (implies (And (interp-st-bfrs-ok interp-st)
+                  (bfr-listp (gl-objectlist-bfrlist new-thenval-stack)
+                             (logicman->bfrstate (interp-st->logicman interp-st))))
+             (interp-st-bfrs-ok (update-interp-st->thenval-stack new-thenval-stack interp-st))))
+
+  (defthm interp-st-bfrs-ok-of-update-elseval-stack
+    (implies (And (interp-st-bfrs-ok interp-st)
+                  (bfr-listp (gl-objectlist-bfrlist new-elseval-stack)
+                             (logicman->bfrstate (interp-st->logicman interp-st))))
+             (interp-st-bfrs-ok (update-interp-st->elseval-stack new-elseval-stack interp-st))))
+
+)
+
+
+
 ;; (define glcp-unify-alist-bfrlist ((x glcp-unify-alist-p))
 ;;   :measure (len (glcp-unify-alist-fix x))
 ;;   (b* ((x (glcp-unify-alist-fix x))
@@ -67,6 +189,27 @@
 (defmacro gl-msg (str &rest args)
   `(glcp-interp-error-message ,str ,(make-fmt-bindings acl2::*base-10-chars* args)))
 
+
+(define gl-interp-store-debug-info (msg obj interp-st state)
+  :returns (new-state)
+  (b* ((stack-obj (stobj-let ((stack (interp-st->stack interp-st)))
+                             (obj)
+                             (stack-extract stack)
+                             obj))
+       (state (f-put-global 'gl-interp-error-message msg state))
+       (state (f-put-global 'gl-interp-error-debug-obj obj state))
+       (state (f-put-global 'gl-interp-error-stack stack-obj state)))
+    state)
+  ///
+  (defret w-of-<fn>
+    (equal (w new-state) (w state))))
+
+(defmacro gl-interp-error (&key msg debug-obj (nvals '1))
+  `(b* ((msg ,msg)
+        (debug-obj ,debug-obj)
+        (state (gl-interp-store-debug-info msg debug-obj interp-st state)))
+     (mv msg ,@(acl2::repeat nvals nil) interp-st state)))
+  
 
 
 ;; (define glcp-interp-error (msg &key (interp-st 'interp-st)
@@ -122,14 +265,14 @@
                                   (args gl-objectlist-p)
                                   (dont-concrete-exec)
                                   state)
-  :returns (mv ok ans)
+  :returns (mv ok (ans gl-object-p))
   (b* (((gl-function-mode mode))
        ((when (or dont-concrete-exec
                   (not (g-concretelist-p args))))
         (mv nil nil))
        ((mv err ans)
         (magic-ev-fncall fn (g-concretelist-vals args) state t nil)))
-    (mv (not err) ans)))
+    (mv (not err) (g-concrete ans))))
 
 
 (def-b*-binder gl-interp-recursive-call
@@ -227,8 +370,7 @@
   (b* (((mv synp-ok synp-term untrans) (match-syntax-bind-synp synp-arg))
        ((unless (and synp-ok (pseudo-term-case x :var)))
         ;; We could go ahead and simulate x anyway but this does seem like an error.
-        (mv (gl-msg "Bad syntax-bind form: args ~x0, ~x1." synp-arg x)
-            nil interp-st state))
+        (gl-interp-error :msg (gl-msg "Bad syntax-bind form: args ~x0, ~x1." synp-arg x)))
        (varname (acl2::pseudo-term-var->name x))
        (bindings (append (interp-st-minor-bindings interp-st)
                          (interp-st-bindings interp-st)))
@@ -237,13 +379,13 @@
        ;; convenient in case we want to bind a variable in different places for
        ;; different cases.  
        ((when (assoc-eq varname bindings))
-        (mv (gl-msg "Syntax-bind error: ~x0 was supposed to be bound in a ~
-                       syntax-bind form but was already bound" varname)
-            nil interp-st state))
+        (gl-interp-error
+         :msg (gl-msg "Syntax-bind error: ~x0 was supposed to be bound in a ~
+                       syntax-bind form but was already bound" varname)))
        ((mv ok val) (acl2::magic-ev synp-term bindings state t t))
        ((unless ok)
-        (mv (gl-msg "Syntax-bind error: ~x0 failed to evaluate -- translated: ~x1" untrans synp-term)
-            nil interp-st state))
+        (gl-interp-error
+         :msg (gl-msg "Syntax-bind error: ~x0 failed to evaluate -- translated: ~x1" untrans synp-term)))
        (val-obj (g-concrete val))
        (interp-st (interp-st-add-binding varname val-obj interp-st)))
     (mv nil val-obj interp-st state)))
@@ -285,7 +427,14 @@
                    (b* ((pathcond (pathcond-rewind checkpoint bfr-mode pathcond)))
                      (mv contra nil pathcond constraint-pathcond))))
                (mv nil checkpoint pathcond constraint-pathcond))
-             (mv contra checkpoint interp-st)))
+             (mv contra checkpoint interp-st))
+  ///
+  (defret interp-st-get-of-interp-st-pathcond-assume
+    (implies (and (not (equal (interp-st-field-fix key) :pathcond))
+                  (not (equal (interp-st-field-fix key) :constraint)))
+             (equal (interp-st-get key new-interp-st)
+                    (interp-st-get key interp-st)))))
+             
 
 
 (define interp-st-pathcond-rewind (checkpoint
@@ -345,7 +494,7 @@
   
 
 
-(define gl-rewrite-relive-hyp-synp ((synp-type symbolp)
+(define gl-rewrite-relieve-hyp-synp ((synp-type symbolp)
                                     (form pseudo-termp)
                                     (vars)
                                     (untrans-form)
@@ -366,8 +515,8 @@
                          (interp-st-bindings interp-st)))
        ((mv ok val) (acl2::magic-ev form bindings state t t))
        ((unless ok)
-        (mv (gl-msg "Synp error: ~x0 failed to evaluate -- translated: ~x1" untrans-form form)
-            nil interp-st state))
+        (gl-interp-error
+         :msg (gl-msg "Synp error: ~x0 failed to evaluate -- translated: ~x1" untrans-form form)))
        ((when (eq synp-type 'syntaxp))
         (mv nil val interp-st state))
        ;; bind-free...
@@ -375,786 +524,1513 @@
         ;; No error -- bind-free evaluated to NIL which means just don't do the rewrite.
         (mv nil nil interp-st state))
        ((unless (gl-object-alist-p val))
-        (mv (gl-msg "Bind-free error: ~x0 evaluated to a non-GL object alist: ~x1" untrans-form val)
-            nil interp-st state))
+        (gl-interp-error
+         :msg (gl-msg "Bind-free error: ~x0 evaluated to a non-GL object alist: ~x1" untrans-form val)))
        (newly-bound-vars (alist-keys bindings))
        ((when (and (symbol-listp vars)
                    (not (subsetp-eq vars newly-bound-vars))))
-        (mv (gl-msg "Bind-free error: ~x0 evaluated to an alist not ~
-                     containing the required vars ~x1: ~x2" untrans-form val vars)
-            nil interp-st state))
+        (gl-interp-error
+         :msg (gl-msg "Bind-free error: ~x0 evaluated to an alist not ~
+                     containing the required vars ~x1: ~x2" untrans-form val vars)))
        ;; Consider allowing already-bound variables to be bound in the new
        ;; bindings, and just omitting them from the final bindings.  Might be
        ;; convenient in case we want to bind a variable in different places for
        ;; different cases.  
        ((when (intersectp-eq (alist-keys val) newly-bound-vars))
-        (mv (gl-msg "Bind-free error: ~x0 evaluated to a non-GL object alist: ~x1" untrans-form val)
-            nil interp-st state))
+        (gl-interp-error
+         :msg (gl-msg "Bind-free error: ~x0 evaluated to a non-GL object alist: ~x1" untrans-form val)))
        (interp-st (interp-st-set-bindings (append val (interp-st-bindings interp-st)) interp-st)))
     (mv nil t interp-st state)))
 
 
 
-(defines gl-interp
-  (define gl-interp-test ((x pseudo-termp)
-                          interp-st
-                          state)
-    ;; Translate a term to a GL object under the given alist substitution, preserving IFF.
-    :measure (list (nfix (interp-st->reclimit interp-st))
-                   12 (pseudo-term-binding-count x) 0)
-    :well-founded-relation acl2::nat-list-<
-    :guard (bfr-listp (glcp-unify-alist-bfrlist alist) (interp-st->bfrstate interp-st))
-    :returns (mv err
-                 (xobj gl-object-p)
-                 new-interp-st
-                 new-state)
-    (b* (((interp-st-bind
-           (equiv-contexts '(iff)))
-          ((gl-interp-recursive-call err xobj interp-st state)
-           (gl-interp-term-equivs x interp-st state)))
-         ((when err)
-          (mv err nil interp-st state)))
-      (gl-interp-simplify-if-test xobj interp-st state)))
-
-  (define gl-interp-term-equivs ((x pseudo-termp)
-                                 interp-st
-                                 state)
-    :measure (list (nfix (interp-st->reclimit interp-st)) 2020 (pseudo-term-binding-count x) 40)
-    :returns (mv err
-                 (xobj gl-object-p)
-                 new-interp-st
-                 new-state)
-    (b* (((mv err xobj interp-st state)
-          (gl-interp-term x interp-st state))
-         ((when err) (mv err nil interp-st state))
-         ((unless (glcp-term-obj-p xobj))
-          (glcp-value xobj))
-         (contexts (interp-st->equiv-contexts interp-st)))
-      (stobj-let ((pathcond (interp-st->pathcond interp-st))
-                  (logicman (interp-st->logicman interp-st))
-                  (bvar-db (interp-st->bvar-db interp-st)))
-                 (replacedp val pathcond)
-                 (try-equivalences-loop
-                  xobj contexts 100 ;; bozo, configure reclimit for try-equivalences-loop?
-                  pathcond bvar-db logicman state)
-                 (glcp-value val))))
-
-  (define gl-interp-term ((x pseudo-termp)
-                          interp-st
-                          state)
-    :measure (list (nfix (interp-st->reclimit interp-st))
-                   2020 (pseudo-term-binding-count x) 20)
-    :returns (mv err
-                 (xobj gl-object-p)
-                 new-interp-st
-                 new-state)
-    (b* ((interp-st (interp-st-fix interp-st)))
-      (pseudo-term-case x
-        :const (glcp-value (g-concrete x.val))
-        :var (b* ((minor-look (assoc-eq x.name (interp-st-minor-bindings interp-st)))
-                  ((when minor-look)
-                   (glcp-value (cdr minor-look))))
-               (glcp-value (cdr (assoc-eq x.name (interp-st-bindings interp-st)))))
-        :lambda
-        (b* (((mv x-bindings body) (lambda-nest-to-bindinglist x))
-             (interp-st (interp-st-push-minor-frame interp-st))
-             (interp-st (interp-st-set-minor-debug x interp-st))
-             ((interp-st-bind
-               (equiv-contexts nil))
-              ((gl-interp-recursive-call err interp-st state)
-               ;; replaces the top of stack with the bindings
-               (gl-interp-bindinglist bindings interp-st state)))
-
-             ((when err)
-              (b* ((interp-st (interp-st-pop-minor-frame interp-st)))
-                (mv err nil interp-st state)))
-             ((mv err val interp-st state)
-              (gl-interp-term-equivs body interp-st state))
-             (interp-st (interp-st-pop-minor-frame interp-st)))
-          (mv err val interp-st state))
-        :fncall 
-        (b* (((when (and** (eq x.fn 'if) (eql (len x.args) 3)))
-              (gl-interp-if/or (first x.args)
-                               (second x.args)
-                               (third x.args)
-                               interp-st state))
-             ((when (and** (eq x.fn 'return-last) (eql (len x.args) 3)))
-              (gl-interp-return-last (first x.args)
-                                     (second x.args)
-                                     (third x.args)
-                                     interp-st state))
-             ((interp-st-bind
-               (equiv-contexts nil))
-              ((gl-interp-recursive-call err interp-st state)
-               ;; pushes the results from the args onto the scratch frame
-               (gl-interp-arglist x.args interp-st state)))
-
-             ((when err)
-              (mv err nil interp-st state)))
-          (gl-interp-fncall x.fn (len x.args) interp-st state)))))
-
-  (define gl-interp-arglist ((args pseudo-term-listp)
-                             interp-st
-                             state)
-    :measure (list (nfix (interp-st->reclimit interp-st))
-                   2020 (pseudo-term-list-binding-count args) 20)
-    :returns (mv err
-                 new-interp-st
-                 new-state)
-    (b* (((when (atom args)) (mv nil interp-st state))
-         ((gl-interp-recursive-call err arg1 interp-st state)
-          (gl-interp-term-equivs (car args) interp-st state))
-         ((when err) (mv err interp-st state))
-         (interp-st (interp-st-push-scratch arg1 interp-st)))
-      (gl-interp-arglist (cdr args) interp-st state)))
-
-  (define gl-interp-bindinglist ((bindings bindinglist-p)
-                                 interp-st
-                                 state)
-    :measure (list (nfix (interp-st->reclimit interp-st))
-                   2020
-                   (bindinglist-count bindings)
-                   20)
-    :returns (mv err
-                 new-interp-st
-                 new-state)
-    (b* (((when (atom bindings)) (mv nil interp-st state))
-         ((binding x1) (car x))
-         ((gl-interp-recursive-call err interp-st state)
-          (gl-interp-arglist x1.args interp-st state))
-         ((when err) (mv err interp-st state))
-         (argslen (len x1.args))
-         (args (interp-st-peek-scratch argslen interp-st))
-         (interp-st (interp-st-pop-scratch argslen interp-st))
-         (interp-st (interp-st-add-minor-bindings (pairlis$ x1.formals args) interp-st)))
-      (gl-interp-bindinglist (cdr bindings) interp-st state)))
-         
-  (define gl-interp-fncall ((fn pseudo-fnsym-p)
-                            (arity natp)
-                            interp-st
-                            state)
-    :measure (list (nfix (interp-st->reclimit interp-st))
-                   0 0 1)
-    :returns (mv err
-                 (ans gl-object-p)
-                 new-interp-st
-                 new-state)
-    (b* (((gl-function-mode fn-mode)
-          (gl-function-mode-fix!
-           (cdr (hons-assoc-equal fn (table-alist 'gl-fn-modes (w state))))))
-         (args (interp-st-peek-scratch arity interp-st))
-         (interp-st (interp-st-pop-scratch arity interp-st))
-         ((mv successp ans)
-          (fncall-try-concrete-eval fn args fn-mode.dont-concrete-exec state))
-         ((when successp)
-          (mv nil ans interp-st state))
-         (reclimit (interp-st->reclimit interp-st))
-         ((when (zp reclimit))
-          (mv (gl-msg "The recursion limit ran out.") nil interp-st state))
-         ((interp-st-bind
-           (reclimit (1- reclimit) reclimit))
-          ((gl-interp-recursive-call err successp ans interp-st state)
-           (gl-rewrite-fncall fn args fn-mode.dont-rewrite interp-st state)))
-         ((when err)
-          (mv err nil interp-st state))
-         ((when successp)
-          (mv nil ans interp-st state))
-         ((mv successp ans interp-st state)
-          (gl-primitive-fncall fn args fn-mode.dont-primitive-exec interp-st state))
-         ((when successp)
-          (mv nil ans interp-st state))
-         ((interp-st-bind
-           (reclimit (1- reclimit) reclimit))
-          ((mv err successp ans interp-st state)
-           (gl-interp-fn-definition fn args fn-mode.dont-expand-def interp-st state)))
-         ((when err)
-          (mv err nil interp-st state))
-         ((when successp)
-          (mv nil ans interp-st state)))
-      (mv nil (g-apply fn args) interp-st state)))
-
-  (define gl-interp-fn-definition ((fn pseudo-fnsym-p)
-                                   (args gl-objectlist-p)
-                                   (dont)
-                                   interp-st
-                                   state)
-    :measure (list (nfix (interp-st->reclimit interp-st)) 20000 0 0)
-    :returns (mv err successp
-                 (ans gl-object-p)
-                 new-interp-st
-                 new-state)
-    (b* (((when dont)
-          (mv nil nil nil interp-st state))
-         ((mv ok body formals)
-          (acl2::fn-get-def fn state))
-         ((unless ok)
-          (mv nil nil nil interp-st state))
-         ((unless (eql (len formals) arity))
-          (mv (gl-msg "Error interpreting a call of ~x0: it was given ~x1 arguments but has ~x2 formals."
-                   fn arity (len formals))
-              nil nil interp-st state))
-         (interp-st (interp-st-push-frame (pairlis$ formals args) interp-st))
-         (interp-st (interp-st-set-debug fn interp-st))
-         ((mv err ans interp-st state)
-          (gl-interp-term-equivs body interp-st state))
-         (interp-st (interp-st-pop-frame interp-st)))
-      (mv err ans interp-st state)))
+;; Used in merge-branches to recognize a branch on which we can unify some
+;; function.  BOZO We might want to try more than one function for some objects
+;; -- e.g. for :g-integer we could do both int and intcons, for concrete values
+;; that are conses we could do both concrete and bool, etc.  Ideally we'd try
+;; all the functions that the argument could unify with.
+(define gl-fncall-object->fn ((x gl-object-p))
+  :returns (fn pseudo-fnsym-p) ;; nil if didn't match
+  (gl-object-case x
+    :g-boolean 'bool
+    :g-integer 'int
+    :g-concrete 'concrete
+    :g-apply x.fn
+    :g-cons 'cons
+    :otherwise nil))
 
 
-  (define gl-rewrite-fncall ((fn pseudo-fnsym-p)
+(defthm base-apply-ev-lst-of-kwote-lst
+  (equal (base-apply-ev-lst (kwote-lst x) a)
+         (true-list-fix x)))
+
+(defthm not-quote-when-pseudo-fnsym-p
+  (implies (pseudo-fnsym-p x)
+           (not (equal x 'quote))))
+
+(define gl-object-recognize-merge-fncall ((x gl-object-p))
+  ;; Note: This is used when we want to merge two calls of the same function,
+  ;; e.g.  (if test (foo x y) (foo w z)).  We don't want to match a g-boolean
+  ;; to (bool x), for example, because that would lead to an infinite loop where we
+  ;; match (if test (g-boolean b) (g-boolean c)) as
+  ;; (if test (bool (g-boolean b)) (bool (g-boolean c)))
+  ;; then merge the args, i.e. (list (g-boolean b)) (list (g-boolean c))
+  ;; in which when we merge the first arg we get back to
+  ;; (if test (g-boolean b) (g-boolean c)) and get stuck in an infinite loop.
+  :returns (mv (fn pseudo-fnsym-p)
+               (args gl-objectlist-p))
+  (gl-object-case x
+    ;; :g-boolean (mv 'bool (list (gl-object-fix x)))
+    ;; :g-integer (mv 'int (list (gl-object-fix x)))
+    ;; :g-concrete (mv 'concrete (list (gl-object-fix x)))
+    :g-apply (mv x.fn x.args)
+    :g-cons (mv 'cons (list x.car x.cdr))
+    :otherwise (mv nil nil))
+  ///
+
+  (defret eval-when-gl-object-recognize-merge-fncall
+    (implies fn
+             (equal (base-apply-ev (cons fn
+                                         (kwote-lst (base-gl-objectlist-eval args env)))
+                                   a)
+                    (base-gl-object-eval x env)))
+    :hints(("Goal" :in-theory (enable base-apply base-gl-objectlist-eval
+                                      base-apply-ev-of-fncall-args))))
+
+  (defret gl-objectlist-count-of-recognize-merge-fncall
+    (implies fn
+             (<= (gl-objectlist-count args) (gl-object-count x)))
+    :hints(("Goal" :in-theory (enable gl-objectlist-count))
+           (and stable-under-simplificationp
+                '(:expand ((gl-object-count x)))))
+    :rule-classes :linear)
+
+  (defret gl-bfr-objectlist-p-of-<fn>
+    (implies (gl-bfr-object-p x)
+             (gl-bfr-objectlist-p args)))
+
+  (defret bfr-listp-gl-objectlist-bfrlist-of-<fn>
+    (implies (bfr-listp (gl-object-bfrlist x))
+             (bfr-listp (gl-objectlist-bfrlist args)))
+    :hints (("goal" :Expand ((gl-object-bfrlist x))))))
+
+;; (define gl-object-recognize-fncall ((x gl-object-p))
+;;   :prepwork ((local (in-theory (enable gl-fncall-object->fn))))
+;;   :returns (mv (fn (equal fn (gl-fncall-object->fn x)))
+;;                (args gl-objectlist-p))
+;;   (gl-object-case x
+;;     :g-boolean (mv 'bool (list (gl-object-fix x)))
+;;     :g-integer (mv 'int (list (gl-object-fix x)))
+;;     :g-concrete (mv 'concrete (list (gl-object-fix x)))
+;;     :g-apply (mv x.fn x.args)
+;;     :g-cons (mv 'cons (list x.car x.cdr))
+;;     :otherwise (mv nil nil))
+;;   ///
+;;   (defret eval-when-gl-object-recognize-fncall
+;;     (implies (gl-fncall-object->fn x)
+;;              (equal (base-gl-object-eval x env)
+;;                     (base-apply (gl-fncall-object->fn x)
+;;                                 (base-gl-objectlist-eval args env))))
+;;     :hints(("Goal" :in-theory (enable base-apply base-gl-objectlist-eval)))))
+
+;; (defthm-base-gl-object-eval-flag
+;;   (defthm base-gl-object-eval-of-gl-bfr-object-fix
+;;     (equal (base-gl-object-eval (gl-bfr-object-fix x (logicman->bfrstate logicman))
+;;                                 env logicman)
+;;            (base-gl-object-eval x env logicman))
+;;     :hints ('(:expand ((base-gl-object-eval x env logicman)
+;;                        (gl-bfr-object-fix x (logicman->bfrstate logicman)))))
+;;     :flag base-gl-object-eval)
+;;   (defthm base-gl-objectlist-eval-of-gl-bfr-object-fix
+;;     (equal (base-gl-objectlist-eval (gl-bfr-objectlist-fix x (logicman->bfrstate logicman))
+;;                                 env logicman)
+;;            (base-gl-objectlist-eval x env logicman))
+;;     :hints ('(:expand ((base-gl-objectlist-eval x env logicman)
+;;                        (gl-bfr-objectlist-fix x (logicman->bfrstate logicman)))))
+;;     :flag base-gl-objectlist-eval))
+
+;; BOZO move
+
+
+
+(define gl-object-basic-merge ((test lbfr-p)
+                               (then gl-object-p)
+                               (else gl-object-p)
+                               &optional
+                               (logicman 'logicman))
+  :returns (mv (obj gl-object-p)
+               new-logicman)
+  :guard-hints (("goal" :in-theory (enable bfr-ite-bss-fn)))
+  :guard (and (gl-bfr-object-p then (logicman->bfrstate))
+              (gl-bfr-object-p else (logicman->bfrstate)))
+  (b* ((bfrstate (logicman->bfrstate)))
+    (gl-object-case then
+      :g-boolean (gl-object-case else
+                   :g-boolean (b* (((mv bfr logicman) (bfr-ite (bfr-fix test)
+                                                               (bfr-fix then.bool)
+                                                               (bfr-fix else.bool))))
+                                (mv (g-boolean bfr) logicman))
+                   :otherwise (mv (gl-bfr-object-fix (g-ite (g-boolean test) then else)) logicman))
+      :g-integer (gl-object-case else
+                   :g-integer (b* (((mv bits logicman) (bfr-ite-bss (bfr-fix test)
+                                                                    (bfr-list-fix then.bits)
+                                                                    (bfr-list-fix else.bits)
+                                                                    logicman)))
+                                (mv (g-integer bits) logicman))
+                   :otherwise (mv (gl-bfr-object-fix (g-ite (g-boolean test) then else)) logicman))
+      :otherwise (mv (gl-bfr-object-fix (g-ite (g-boolean test) then else)) logicman)))
+  ///
+  (defret gl-bfr-object-p-of-<fn>
+    (gl-bfr-object-p obj (logicman->bfrstate new-logicman)))
+
+  (defret eval-of-gl-object-basic-merge
+    (equal (base-gl-object-eval obj env new-logicman)
+           (if (gobj-bfr-eval test env)
+               (base-gl-object-eval then env logicman)
+             (base-gl-object-eval else env logicman)))
+    :hints(("Goal" 
+            :in-theory (enable gobj-bfr-eval gobj-bfr-list-eval-is-bfr-list-eval))))
+
+  (defret logicman-extension-p-of-<fn>
+    (logicman-extension-p new-logicman logicman))
+  
+  (local (defthm gl-bfr-objectlist-of-gl-bfr-object-fix
+           (bfr-listp (gl-object-bfrlist (gl-bfr-object-fix x bfrstate)) bfrstate)
+           :hints (("goal" :use ((:instance bfr-listp-of-gl-object-bfrlist
+                                  (x (gl-bfr-object-fix x bfrstate))))))))
+
+  (defret bfr-listp-of-gl-object-basic-merge
+    ;; (implies (and (lbfr-p test)
+    ;;               (lbfr-listp (gl-object-bfrlist thenval))
+    ;;               (lbfr-listp (gl-object-bfrlist elseval)))
+             (bfr-listp (gl-object-bfrlist obj) (logicman->bfrstate new-logicman))))
+
+
+(define gl-int-primitive ((args gl-objectlist-p) interp-st state)
+  :returns (mv successp
+               (ans gl-object-p)
+               interp-st
+               state)
+  (if (eql (len args) 1)
+      (let ((x (car args)))
+        (gl-object-case x
+          :g-integer (mv t (gl-object-fix x) interp-st state)
+          :otherwise (mv nil nil interp-st state)))
+    (mv nil nil interp-st state)))
+
+(define gl-endint-primitive ((args gl-objectlist-p) interp-st state)
+  :returns (mv successp
+               (ans gl-object-p)
+               interp-st
+               state)
+  (if (eql (len args) 1)
+      (let ((x (car args)))
+        (gl-object-case x
+          :g-boolean (mv t (g-integer (list x.bool)) interp-st state)
+          :otherwise (mv nil nil interp-st state)))
+    (mv nil nil interp-st state)))
+
+(define gl-intcons-primitive ((args gl-objectlist-p) interp-st state)
+  :returns (mv successp
+               (ans gl-object-p)
+               interp-st
+               state)
+  (if (eql (len args) 2)
+      (b* (((list car cdr) args))
+        (gl-object-case car
+          :g-boolean (gl-object-case cdr
+                       :g-integer (mv t (g-integer (cons car.bool cdr.bits)) interp-st state)
+                       :otherwise (mv nil nil interp-st state))
+          :otherwise (mv nil nil interp-st state)))
+    (mv nil nil interp-st state)))
+
+(define gl-intcar-primitive ((args gl-objectlist-p) interp-st state)
+  :returns (mv successp
+               (ans gl-object-p)
+               interp-st
+               state)
+  (if (eql (len args) 1)
+      (let ((x (car args)))
+        (gl-object-case x
+          :g-integer (mv t (g-boolean (car x.bits)) interp-st state)
+          :otherwise (mv nil nil interp-st state)))
+    (mv nil nil interp-st state)))
+
+(define gl-intcdr-primitive ((args gl-objectlist-p) interp-st state)
+  :returns (mv successp
+               (ans gl-object-p)
+               interp-st
+               state)
+  (if (eql (len args) 1)
+      (let ((x (car args)))
+        (gl-object-case x
+          :g-integer (mv t (g-integer (cdr x.bits)) interp-st state)
+          :otherwise (mv nil nil interp-st state)))
+    (mv nil nil interp-st state)))
+
+(define gl-bool-primitive ((args gl-objectlist-p) interp-st state)
+  :returns (mv successp
+               (ans gl-object-p)
+               interp-st
+               state)
+  (if (eql (len args) 1)
+      (let ((x (car args)))
+        (gl-object-case x
+          :g-boolean (mv t (gl-object-fix x) interp-st state)
+          :otherwise (mv nil nil interp-st state)))
+    (mv nil nil interp-st state)))
+
+(define gl-primitive-fncall ((fn pseudo-fnsym-p)
                              (args gl-objectlist-p)
                              (dont)
                              interp-st
                              state)
-    :measure (list (nfix (interp-st->reclimit interp-st)) 20000 0 0)
-    :returns (mv err successp
-                 (ans gl-object-p)
-                 new-interp-st
-                 new-state)
-    (b* (((when dont)
-          (mv nil nil nil interp-st state))
-         (rules (fn-rewrite-rules fn (glcp-config->rewrite-rule-table
-                                      (interp-st->config interp-st))
-                                  (w state)))
-         ((unless rules)
-          (mv nil nil nil interp-st state))
-         (reclimit (interp-st->reclimit interp-st))
-         ((when (zp reclimit))
-          (mv (gl-msg "The recursion limit ran out.")
-              nil nil interp-st state)))
-      (gl-rewrite-try-rules rules fn args interp-st state)))
-
-  (define gl-rewrite-try-rules ((rules pseudo-rewrite-rule-listp)
-                                (fn pseudo-fnsym-p)
-                                (args gl-objectlist-p)
-                                interp-st
-                                state)
-    :measure (list (nfix (interp-st->reclimit interp-st)) 10000 (len rules) 0)
-    :returns (mv err successp
-                 (ans gl-object-p)
-                 new-interp-st
-                 new-state)
-    (b* (((when (atom rules))
-          (mv nil nil nil interp-st state))
-         ((gl-interp-recursive-call err successp ans interp-st state)
-          (gl-rewrite-try-rule (car rules) fn args interp-st state))
-         ((when (or err successp))
-          (mv err successp ans interp-st state)))
-      (gl-rewrite-try-rules (cdr rules) fn args interp-st state)))
-
-  (define gl-rewrite-try-rule ((rule pseudo-rewrite-rule-p)
-                               (fn pseudo-fnsym-p)
-                               (args gl-objectlist-p)
-                               interp-st
-                               state)
-    :measure (list (nfix (interp-st->reclimit interp-st)) 10000 0 0)
-    :returns (mv err successp
-                 (ans gl-object-p)
-                 new-interp-st
-                 new-state)
-    (b* (((acl2::rewrite-rule rule))
-         ((unless (and** (mbt (and* (symbolp rule.equiv)
-                                    (not (eq rule.equiv 'quote))
-                                    ;; (ensure-equiv-relationp rule.equiv (w state))
-                                    (not (eq rule.subclass 'acl2::meta))
-                                    (pseudo-termp rule.lhs)))
-                         (pseudo-term-case rule.lhs :fncall (eq rule.lhs.fn (pseudo-fnsym-fix fn)))))
-          (mv (gl-msg "Malformed rewrite rule: ~x0~%" rule)
-              nil nil interp-st state))
-         ((unless (or (eq rule.equiv 'equal)
-                      ;; bozo check refinements
-                      (member rule.equiv (interp-st->equiv-contexts interp-st))))
-          (mv nil nil nil interp-st state))
-         (rule.lhs.args (pseudo-term-call->args rule.lhs))
-         ((mv unify-ok bindings) (glcp-unify-term/gobj-list rule.lhs.args args nil))
-         ((unless unify-ok) (mv nil nil nil interp-st state))
-         ((unless (mbt (pseudo-term-listp rule.hyps)))
-          (mv (gl-msg "Malformed rewrite rule: ~x0~%" rule)
-              nil nil interp-st state))
-         (backchain-limit (interp-st->backchain-limit interp-st))
-         ((when (and* rule.hyps (eql 0 backchain-limit)))
-          (mv nil nil nil interp-st state))
-         (flags (interp-st->flags interp-st))
-         (hyps-flags  (!interp-st->intro-bvars
-                       t
-                       (!interp-flags->intro-bvars
-                        nil
-                        (!interp-flags->simplify-logic nil flags))))
-         (interp-st (interp-st-push-frame bindings interp-st))
-         (interp-st (interp-st-set-debug rule interp-st))
-         ((interp-st-bind
-           (flags hyps-flags flags)
-           (contexts '(iff))
-           (backchain-limit (1- backchain-limit) backchain-limit))
-          ((gl-interp-recursive-call err successp interp-st state)
-           (gl-rewrite-relieve-hyps rule.hyps interp-st state)))
-
-         ((unless successp)
-          (b* ((interp-st (interp-st-pop-frame interp-st)))
-            (mv err nil nil interp-st state)))
-
-         (concl-flags (!interp-st->intro-bvars t flags))
-         ((interp-st-bind
-           (flags concl-flags flags))
-          ((mv err val interp-st state)
-           (gl-interp-term-equivs rule.rhs interp-st state)))
-
-         (interp-st (interp-st-pop-frame interp-st)))
-
-      (mv err (not err) val interp-st state)))
-          
-  (define gl-rewrite-relieve-hyps ((hyps pseudo-term-listp)
-                                   interp-st
-                                   state)
-    :measure (list (nfix (interp-st->reclimit interp-st)) 9000
-                   (pseudo-term-list-binding-count hyps) 0)
-    :returns (mv err successp
-                 new-interp-st
-                 new-state)
-    (b* (((when (atom hyps))
-          (mv nil t interp-st state))
-         ((mv err ok interp-st state)
-          (gl-rewrite-relieve-hyp (car hyps) interp-st state))
-         ((when (or err (not ok)))
-          (mv err ok interp-st state)))
-      (gl-rewrite-relieve-hyps (cdr hyps) interp-st state)))
-
-  (define gl-rewrite-relieve-hyp ((hyp pseudo-termp)
-                                  interp-st
-                                  state)
-    :measure (list (nfix (interp-st->reclimit interp-st)) 9000
-                   (pseudo-term-binding-count hyp) 0)
-    :returns (mv err successp
-                 new-interp-st
-                 new-state)
-    (b* (((mv synp-type untrans-form trans-term vars)
-          (gl-interp-match-synp hyp))
-         ((when synp-type)
-          (gl-rewrite-relieve-hyp-synp synp-type trans-term interp-st state))
-         ((mv err test-bfr interp-st state)
-          (gl-interp-test hyp interp-st state)))
-      (mv err (eq test-bfr t) interp-st state)))
-
-  (define gl-interp-time$ ((timing-arg pseudo-termp)
-                           (x pseudo-termp)
-                           interp-st
-                           state)
-    :measure (list (nfix (interp-st->reclimit interp-st)) 2020
-                   (+ (pseudo-term-binding-count first-arg)
-                      (pseudo-term-binding-count last-arg))
-                   30)
-    :returns (mv err
-                 (ans gl-object-p)
-                 new-interp-st
-                 new-state)
-    (b* (((interp-st-bind
-           (equiv-contexts nil))
-          ((gl-interp-recursive-call err time$-arg interp-st state)
-           (gl-interp-term-equivs timing-arg interp-st state)))
-         ((when err)
-          (mv err nil interp-st state))
-         (time$-arg (gl-interp-time$-arg time$-arg x)))
-      (time$1 time$-arg
-              (gl-interp-term-equivs x interp-st state))))
-         
-  (define gl-interp-return-last ((return-last-fnname pseudo-termp)
-                                 (first-arg pseudo-termp)
-                                 (last-arg pseudo-termp)
-                                 interp-st state)
-    :measure (list (nfix (interp-st->reclimit interp-st)) 2020
-                   (+ (pseudo-term-binding-count first-arg)
-                      (pseudo-term-binding-count last-arg))
-                   40)
-    :returns (mv err
-                 (ans gl-object-p)
-                 new-interp-st
-                 new-state)
-    (b* (((when (equal return-last-fnname ''time$1-raw))
-          (gl-interp-time$ first-arg last-arg interp-st state))
-         ((when (equal return-last-fnname ''(syntax-bind)))
-          (gl-interp-syntax-bind first-arg last-arg interp-st state)))
-      ;; Otherwise just evaluate the last-arg.
-      (gl-interp-term-equivs last-arg interp-st state)))
-                
-               
-
-  (define gl-interp-if/or ((test pseudo-termp)
-                           (then pseudo-termp)
-                           (else pseudo-termp)
-                           interp-st
-                           state)
-    :measure (list (nfix (interp-st->reclimit interp-st))
-                   2020
-                   (+ (pseudo-term-binding-count test)
-                      (pseudo-term-binding-count then)
-                      (pseudo-term-binding-count else))
-                   60)
-    :returns (mv err
-                 (ans gl-object-p)
-                 new-interp-st
-                 new-state)
-    (if (hons-equal test then)
-        (gl-interp-or test else interp-st state)
-      (gl-interp-if test then else interp-st state)))
-
-  
-  (define gl-interp-if ((test pseudo-termp)
-                        (then pseudo-termp)
-                        (else pseudo-termp)
-                        interp-st
-                        state)
-    :measure (list (nfix (interp-st->reclimit interp-st))
-                   2020
-                   (+ (pseudo-term-binding-count test)
-                      (pseudo-term-binding-count then)
-                      (pseudo-term-binding-count else))
-                   40)
-    :returns (mv err
-                 (ans gl-object-p)
-                 new-interp-st
-                 new-state)
-    ;; Tricky because we have to keep the test/thenval on the stack while we
-    ;; run the then/else branches, because we might simplify the logicman while
-    ;; running them.
-    (b* (((gl-interp-recursive-call err testbfr interp-st state)
-          (gl-interp-test test interp-st state))
-         ((when err) (mv err nil interp-st state))
-         (interp-st (interp-st-push-bool-scratch testbfr interp-st))
-         ((gl-interp-recursive-call err then-unreachable thenval interp-st state)
-         ;; pushes val onto scratch if not unreachable
-          (gl-maybe-interp testbfr then interp-st state))
-         ((when err)
-          (b* ((interp-st (interp-st-pop-bool-scratch 1 interp-st)))
-            (mv err nil interp-st state)))
-         (interp-st (interp-st-push-scratch thenval interp-st))
-         ;; note: testbool may have changed if we simplified the logicman
-         (testbfr (first (interp-st-bool-scratch interp-st)))
-         ((gl-interp-recursive-call err else-unreachable elseval interp-st state)
-          ;; pushes val onto scratch if not unreachable
-          (gl-maybe-interp (interp-st-bfr-not testbfr) else interp-st state))
-         ((when err)
-          (b* ((interp-st (interp-st-pop-scratch 1 interp-st))
-               (interp-st (interp-st-pop-bool-scratch 1 interp-st)))
-            (mv err nil interp-st state)))
-         (thenval (first (interp-st-scratch interp-st)))
-         (testbfr (first (interp-st-bool-scratch interp-st)))
-         (interp-st (interp-st-pop-scratch 1 interp-st))
-         (interp-st (interp-st-pop-bool-scratch 1 interp-st))
-         ((when then-unreachable)
-          (if else-unreachable
-              (mv :unreachable nil interp-st state)
-            (mv nil elseval interp-st state)))
-         ((when else-unreachable)
-          (mv nil thenval interp-st state)))
-      (gl-interp-merge-branches testbfr thenval elseval interp-st state)))
-
-  (define gl-interp-or ((test pseudo-termp)
-                        (else pseudo-termp)
-                        interp-st
-                        state)
-    :measure (list (nfix (interp-st->reclimit interp-st))
-                   2020
-                   (+ (pseudo-term-binding-count test)
-                      (pseudo-term-binding-count else))
-                   40)
-    :returns (mv err
-                 (ans gl-object-p)
-                 new-interp-st
-                 new-state)
-    (b* ((equiv-contexts (interp-st->equiv-contexts interp-st))
-         (or-test-equiv-contexts (gl-interp-or-test-equiv-contexts equiv-contexts))
-         ((interp-st-let
-           (equiv-contexts or-test-equiv-contexts equiv-contexts))
-          ((gl-interp-recursive-call err testval interp-st state)
-           (gl-interp-term-equivs test interp-st state)))
-         ((when err) (mv err nil interp-st state))
-         ((mv err testbfr interp-st state)
-          (gl-interp-simplify-if-test testval interp-st state))
-         ((when err) (mv err nil interp-st state))
-         (interp-st (interp-st-push-scratch testval interp-st))
-         (interp-st (interp-st-push-bool-scratch testbfr interp-st))
-         ((gl-interp-recursive-call err else-unreachable elseval interp-st state)
-          ;; pushes val onto scratch if not unreachable
-          (gl-maybe-interp (interp-st-bfr-not testbfr) else interp-st state))
-         (testval (first (interp-st-scratch interp-st)))
-         (testbfr (first (interp-st-bool-scratch interp-st)))
-         (interp-st (interp-st-pop-scratch 1 interp-st))
-         (interp-st (interp-st-pop-bool-scratch 1 interp-st))
-         ((when err)
-          (mv err nil interp-st state))
-         ((when else-unreachable)
-          (mv nil testval interp-st state)))
-      (gl-interp-merge-branches testbfr testval elseval interp-st state)))
+  :returns (mv successp
+               (ans gl-object-p)
+               interp-st
+               state)
+  (if dont
+      (mv nil nil interp-st state)
+    (case (pseudo-fnsym-fix fn)
+      (int (gl-int-primitive args interp-st state))
+      (intcons (gl-intcons-primitive args interp-st state))
+      (intcons* (gl-intcons-primitive args interp-st state))
+      (endint (gl-endint-primitive args interp-st state))
+      (intcar (gl-intcar-primitive args interp-st state))
+      (intcdr (gl-intcdr-primitive args interp-st state))
+      (bool (gl-bool-primitive args interp-st state))
+      (otherwise (mv nil nil interp-st state)))))
+      
 
 
-  (define gl-maybe-interp ((test interp-st-bfr-p)
-                           (x pseudo-termp)
-                           interp-st
-                           state)
-    :measure (list (nfix (interp-st->reclimit interp-st))
-                   2020
-                   (pseudo-term-binding-count x)
-                   40)
-    :returns (mv err
-                 unreachable
-                 (ans gl-object-p)
-                 new-interp-st
-                 new-state)
-    (b* (((mv contra checkpoint interp-st)
-          (interp-st-pathcond-assume test interp-st))
-         ((when contra)
-          (mv nil t nil interp-st state))
-         ((mv err ans interp-st state)
-          (gl-interp-term-equivs x interp-st state))
-         (interp-st (stobj-let ((logicman (interp-st->logicman interp-st))
-                                (pathcond (interp-st->pathcond interp-st)))
-                               (pathcond)
-                               (pathcond-rewind checkpoint (logicman->bfr-mode logicman) pathcond)
-                               interp-st))
-         ((when (eq err :unreachable))
-          (mv nil t nil interp-st state)))
-      (mv err nil ans interp-st state)))
 
-  (define gl-interp-maybe-simplify-if-test ((test interp-st-bfr-p)
-                                            (xobj gl-object-p)
-                                            interp-st
-                                            state)
-    :measure (list (nfix (interp-st->reclimit interp-st))
-                   2000
-                   (gl-object-count xobj)
-                   60)
-    :returns (mv err
-                 unreachable
-                 xbfr
-                 new-interp-st
-                 new-state)
-    (b* (((mv contra checkpoint interp-st)
-          (interp-st-pathcond-assume test interp-st))
-         ((when contra)
-          (mv nil t nil interp-st state))
-         ((mv err ans interp-st state)
-          (gl-interp-simplify-if-test x interp-st state))
-         (interp-st (stobj-let ((logicman (interp-st->logicman interp-st))
-                                (pathcond (interp-st->pathcond interp-st)))
-                               (pathcond)
-                               (pathcond-rewind checkpoint (logicman->bfr-mode logicman) pathcond)
-                               interp-st))
-         ((when (eq err :unreachable))
-          (mv nil t nil interp-st state)))
-      (mv err nil ans interp-st state)))
-
-  (define gl-interp-simplify-if-test ((xobj gl-object-p)
-                                      interp-st
-                                      state)
-    :returns (mv err
-                 xbfr
-                 new-interp-st
-                 new-state)
-    :measure (list (nfix (interp-st->reclimit interp-st))
-                   2000
-                   (gl-object-count xobj)
-                   40)
-    (gl-object-case xobj
-      :g-concrete (mv nil (and xobj.val t) interp-st state)
-      :g-boolean (mv nil xobj.bool interp-st state)
-      :g-integer (mv nil t interp-st state)
-      :g-cons (mv nil t interp-st state)
-      :g-var (stobj-let ((bvar-db (interp-st->bvar-db interp-st))
-                         (logicman (interp-st->logicman interp-st)))
-                        (bfr bvar-db)
-                        (b* (((mv bvar bvar-db) (add-term-bvar-unique xobj bvar-db))
-                             (bvar-db (maybe-add-equiv-term xobj bvar bvar-db state))
-                             (bfr (bfr-var bvar)))
-                          (mv bfr bvar-db))
-                        (mv nil bfr interp-st state))
-      :g-ite (b* (((mv err test-bfr interp-st state)
-                   (gl-interp-simplify-if-test xobj.test interp-st state))
-                  (interp-st (interp-st-push-bool-scratch test-bfr interp-st))
-                  ((gl-interp-recursive-call err then-unreachable then-bfr interp-st state)
-                   (gl-interp-maybe-simplify-if-test test-bfr xobj.then interp-st state))
-                  ((when err)
-                   (b* ((interp-st (interp-st-pop-bool-scratch 1 interp-st)))
-                     (mv err nil interp-st state)))
-                  (test-bfr (car (interp-st-bool-scratch interp-st)))
-                  (interp-st (interp-st-push-bool-scratch then-bfr interp-st))
-                  ((mv err else-unreachable else-bfr interp-st state)
-                   (gl-interp-maybe-simplify-if-test test-bfr xobj.else interp-st state))
-                  ((when err)
-                   (b* ((interp-st (interp-st-pop-bool-scratch 2 interp-st)))
-                     (mv err nil interp-st state)))
-                  (then-bfr (car (interp-st-bool-scratch interp-st)))
-                  (test-bfr (cadr (interp-st-bool-scratch interp-st)))
-                  ((when then-unreachable)
-                   (if else-unreachable
-                       (mv :unreachable nil interp-st state)
-                     (mv nil else-bfr interp-st state)))
-                  ((when else-unreachable)
-                   (mv nil then-bfr interp-st state))
-                  ((mv ite interp-st) (stobj-let ((logicman (interp-st->logicman interp-st)))
-                                                 (ite logicman)
-                                                 (bfr-ite test-bfr then-bfr else-bfr)
-                                                 (mv ite interp-st))))
-               (mv nil ite interp-st state))
-      :g-apply (gl-interp-simplify-if-test-fncall xobj.fn xobj.args interp-st state)))
-
-  (define gl-interp-simplify-if-test-fncall ((x gl-object-p)
-                                             interp-st
-                                             state)
-    :guard (gl-object-case x :g-apply)
-    :measure (list (nfix (interp-st->reclimit interp-st))
-                   2000
-                   (gl-object-count x)
-                   20)
-    :returns (mv err
-                 xbfr
-                 new-interp-st
-                 new-state)
-    (b* (((mv not-matched neg-arg)
-          (gl-apply-match-not x))
-         ((when not-matched)
-          (b* (((mv err bfr interp-st state)
-                (gl-interp-simplify-if-test neg-arg interp-st state))
-               ((when err)
-                (mv err nil interp-st state)))
-            (mv nil (interp-st-bfr-not bfr) interp-st state)))
-         ((g-apply x))
-         ((gl-function-mode fn-mode)
-          (gl-function-mode-fix!
-           (cdr (hons-assoc-equal fn (table-alist 'gl-fn-modes (w state))))))
-
-         ;; BOZO support gl-interp-force-check.
-
-         ;; We rewrite this fncall again because it presumably might not have
-         ;; been done in IFF context before.  E.g.
-         ;; (let ((a (foo x)))
-         ;;   (if a y z))
-         ;; Note we wouldn't do this fully "right" even if we had perfect
-         ;; knowledge of congruences because our test term might be bound to a
-         ;; variable that is used in both Boolean and non-Boolean contexts.
-         ((when (zp reclimit))
-          (mv (gl-msg "The recursion limit ran out.") nil interp-st state))
-         ((interp-st-bind
-           (reclimit (1- reclimit) reclimit)
-           (equiv-contexts '(iff)))
-          ((gl-interp-recursive-call err successp ans interp-st state)
-           (gl-rewrite-fncall x.fn x.args fn-mode.dont-rewrite-under-if-test interp-st state)))
-         ((when err)
-          (mv err nil interp-st state))
-         ((when successp)
-          (b* (((interp-st-bind
-                 (reclimit (1- reclimit) reclimit)))
-               ((mv err ans interp-st state)
-                (gl-interp-simplify-if-test ans interp-st state)))
-            (mv err ans interp-st state)))
-
-         (look (get-term->bvar x bvar-db))
-         ((when look)
-          (b* ((bfr (stobj-let ((logicman (interp-st->logicman interp-st)))
-                               (bfr)
-                               (bfr-var look)
-                               bfr)))
-            (mv nil bfr interp-st state)))
-
-         ((unless (interp-flags->intro-bvars (interp-st->flags interp-st)))
-          ;; Note: we only return intro-bvars-fail when this flag is set to
-          ;; false, which it is not at the top level.  So when we set the flag
-          ;; to true (as we do in relieve-hyp and add-bvar-constraint-substs,
-          ;; e.g.) we check for this error specifically and catch it.
-          ;; Otherwise we expect callers not to set intro-bvars to nil and then
-          ;; they won't have to deal with this error specially.
-          (mv :intro-bvars-fail nil interp-st state))
-
-         ((mv bfr interp-st)
-          (stobj-let ((bvar-db (interp-st->bvar-db interp-st))
-                      (logicman (interp-st->logicman interp-st))
-                      (constraint-db (interp-st->constraint-db interp-st)))
-                     (var bvar-db)
-                     (b* ((bvar (next-bvar bvar-db))
-                          (bvar-db (add-term-bvar x bvar-db))
-                          (bvar-db (maybe-add-equiv-term x bvar bvar-db state))
-                          (bfr (bfr-var bvar)))
-                       (mv bfr bvar-db))
-                     (mv bfr interp-st)))
-
-         ((mv err interp-st state)
-          (gl-interp-add-constraints constraint-substs interp-st state))
-
-         ((when err)
-          (mv err nil interp-st state)))
-      (mv nil bfr interp-st state)))
+(define glcp-unify-term/gobj-list-prefix ((pat pseudo-term-listp)
+                                        (x gl-objectlist-p)
+                                        (alist gl-object-alist-p))
+  ;; Same as glcp-unify-term/gobj-list but doesn't complain about extra or missing elements of x.
+  ;; Equivalent to (glcp-unify-term/gobj-list pat (take (len pat) x) alist).
+  (b* (((when (atom pat)) (mv t (gl-object-alist-fix alist)))
+       ((mv ok alist) (glcp-unify-term/gobj (car pat) (car x) alist))
+       ((unless ok) (mv nil nil)))
+    (glcp-unify-term/gobj-list-prefix (cdr pat) (cdr x) alist))
+  ///
+  (defthm glcp-unify-term/gobj-list-prefix-elim
+    (equal (glcp-unify-term/gobj-list-prefix pat x alist)
+           (glcp-unify-term/gobj-list pat (take (len pat) x) alist))
+    :hints(("Goal" :induct (glcp-unify-term/gobj-list-prefix pat x alist)
+            :expand ((:free (x) (glcp-unify-term/gobj-list pat x alist))
+                     (take (len pat) x))))))
 
 
-  (define gl-interp-add-constraints ((x gl-object-p)
-                                     interp-st
+
+
+
+
+
+
+
+
+
+
+
+
+
+
+
+
+
+
+(local (defthm len-equal-0
+         (equal (equal (len x) 0)
+                (not (consp x)))))
+
+(local
+ (defthm pseudo-term-bindinglist-count-when-consp
+   (implies (consp x)
+            (< (+ (pseudo-term-binding-count (car x))
+                  (pseudo-term-list-binding-count (cdr x)))
+               (pseudo-term-list-binding-count x)))
+    :rule-classes :linear))
+
+(local (defthm len-of-cons
+         (equal (len (cons a b))
+                (+ 1 (len b)))))
+
+(local (defthm and*-hyp
+         (implies (acl2::rewriting-negative-literal `(acl2::binary-and* ,a ,b))
+                  (iff (and* a b) (and a b)))))
+
+(local (defun len-is (x n)
+         (if (zp n)
+             (and (eql n 0) (atom x))
+           (and (consp x)
+                (len-is (cdr x) (1- n))))))
+
+(local (defthm open-len-is
+         (implies (syntaxp (quotep n))
+                  (equal (len-is x n)
+                         (if (zp n)
+                             (and (eql n 0) (atom x))
+                           (and (consp x)
+                                (len-is (cdr x) (1- n))))))))
+                         
+
+(local (defthm equal-len-hyp
+         (implies (syntaxp (or (acl2::rewriting-negative-literal-fn `(equal (len ,x) ,n) mfc state)
+                               (acl2::rewriting-negative-literal-fn `(equal ,n (len ,x)) mfc state)))
+                  (equal (equal (len x) n)
+                         (len-is x n)))))
+
+(local (defthm gl-object-count-of-car-weak
+         (<= (gl-object-count (car x)) (gl-objectlist-count x))
+         :hints (("goal" :cases ((consp x))))
+         :rule-classes :linear))
+
+(local (defthm gl-objectlist-count-of-cdr-weak
+         (<= (gl-objectlist-count (cdr x)) (gl-objectlist-count x))
+         :hints (("goal" :cases ((consp x))))
+         :rule-classes :linear))
+
+(local (defthm mv-nth-of-cons
+         (equal (mv-nth n (cons a b))
+                (if (zp n) a (mv-nth (1- n) b)))
+         :hints(("Goal" :in-theory (enable mv-nth)))))
+
+(defthm gl-object-alist-p-of-stack$a-bindings
+  (gl-object-alist-p (stack$a-bindings stack)))
+
+(defthm gl-object-alist-p-of-stack$a-minor-bindings
+  (gl-object-alist-p (stack$a-minor-bindings stack)))
+
+(defthm gl-object-alist-p-of-stack$a-scratch
+  (gl-objectlist-p (stack$a-scratch stack)))
+
+(local (in-theory (disable (tau-system) len default-car default-cdr
+                           STACK$A-PUSH-BOOL-SCRATCH
+                           STACK$A-POP-SCRATCH
+                           STACK$A-PUSH-SCRATCH
+                           STACK$A-POP-BOOL-SCRATCH
+                           STACK$A-SET-BINDINGS
+                           STACK$A-SET-DEBUG
+                           STACK$A-SET-MINOR-DEBUG
+                           STACK$A-SET-MINOR-BINDINGS
+                           STACK$A-POP-FRAME
+                           STACK$A-PUSH-FRAME
+                           STACK$A-PUSH-MINOR-FRAME
+                           STACK$A-BOOL-SCRATCH
+                           STACK$A-POP-MINOR-FRAME
+                           STACK$A-ADD-MINOR-BINDINGS
+                           STACK$A-MINOR-BINDINGS
+                           STACK$A-SCRATCH
+                           STACK$A-BINDINGS
+                           pseudo-termp
+                           pseudo-term-listp
+                           fgetprop
+                           not
+                           acl2::nfix-when-not-natp
+                           equal-of-booleans-rewrite
+                           mv-nth-cons-meta)))
+
+(set-state-ok t)
+
+(progn
+  (with-output
+    :off (event prove)
+    (defines gl-interp
+        :flag-local nil
+      (define gl-interp-test ((x pseudo-termp)
+                              (interp-st interp-st-bfrs-ok)
+                              state)
+        ;; Translate a term to a GL object under the given alist substitution, preserving IFF.
+        :measure (list (nfix (interp-st->reclimit interp-st))
+                       2020 (pseudo-term-binding-count x) 60)
+        :well-founded-relation acl2::nat-list-<
+        :verify-guards nil
+        :measure-debug t
+        ;; :guard (bfr-listp (gl-object-alist-bfrlist alist) (interp-st->bfrstate interp-st))
+        :returns (mv err
+                     xbfr
+                     new-interp-st
+                     new-state)
+        (b* (((interp-st-bind
+               (equiv-contexts '(iff)))
+              ((gl-interp-recursive-call err xobj interp-st state)
+               (gl-interp-term-equivs x interp-st state)))
+             ((when err)
+              (mv err nil interp-st state)))
+          (gl-interp-simplify-if-test xobj interp-st state)))
+
+      (define gl-interp-term-equivs ((x pseudo-termp)
+                                     (interp-st interp-st-bfrs-ok)
                                      state)
-    :guard (gl-object-case x :g-apply)
-    :measure (list (nfix (interp-st->reclimit interp-st))
-                   2000
-                   (gl-object-count x)
-                   15)
-    :returns (mv err
-                 new-interp-st
-                 new-state)
-    (b* ((constraint-db (interp-st->constraint-db interp-st))
-         ((mv constraint-substs constraint-db)
-          (gbc-process-new-lit x constraint-db state))
-         (interp-st (update-interp-st->constraint-db constraint-db))
-         ((unless constraint-substs)
-          (mv nil interp-st state))
-         ;; Disable the pathcond so that constraint thms are simulated in an empty (universal) context.
-         ((mv pathcond-enabledp interp-st) (stobj-let ((pathcond (interp-st->pathcond interp-st)))
-                                                      (enabledp pathcond)
-                                                      (b* ((enabledp (pathcond-enabledp pathcond))
-                                                           (pathcond (update-pathcond-enabledp nil pathcond)))
-                                                        (mv enabledp pathcond))
-                                                      (mv enabledp interp-st)))
-         ((mv err interp-st state)
-          (gl-interp-add-constraints-for-substs constraint-substs interp-st state))
-         (interp-st (stobj-let ((pathcond (interp-st->pathcond interp-st)))
-                               (pathcond)
-                               (update-pathcond-enabledp pathcond-enabledp pathcond)
-                               interp-st)))
-      (mv err interp-st state)))
-                                                        
+        :measure (list (nfix (interp-st->reclimit interp-st)) 2020 (pseudo-term-binding-count x) 40)
+        :returns (mv err
+                     (xobj gl-object-p)
+                     new-interp-st
+                     new-state)
+        (b* (((mv err xobj interp-st state)
+              (gl-interp-term x interp-st state))
+             ((when err) (mv err nil interp-st state))
+             ((unless (glcp-term-obj-p xobj))
+              (glcp-value xobj))
+             (contexts (interp-st->equiv-contexts interp-st)))
+          (stobj-let ((pathcond (interp-st->pathcond interp-st))
+                      (logicman (interp-st->logicman interp-st))
+                      (bvar-db (interp-st->bvar-db interp-st)))
+                     (replacedp val pathcond)
+                     (try-equivalences-loop
+                      xobj contexts 100 ;; bozo, configure reclimit for try-equivalences-loop?
+                      pathcond bvar-db logicman state)
+                     (glcp-value val))))
+
+      (define gl-interp-term ((x pseudo-termp)
+                              (interp-st interp-st-bfrs-ok)
+                              state)
+        :measure (list (nfix (interp-st->reclimit interp-st))
+                       2020 (pseudo-term-binding-count x) 20)
+        :returns (mv err
+                     (xobj gl-object-p)
+                     new-interp-st
+                     new-state)
+        (pseudo-term-case x
+          :const (glcp-value (g-concrete x.val))
+          :var (b* ((minor-look (assoc-eq x.name (interp-st-minor-bindings interp-st)))
+                    ((when minor-look)
+                     (glcp-value (cdr minor-look))))
+                 (glcp-value (cdr (assoc-eq x.name (interp-st-bindings interp-st)))))
+          :lambda
+          (b* (((mv x-bindings body) (lambda-nest-to-bindinglist x))
+               (interp-st (interp-st-push-minor-frame interp-st))
+               (interp-st (interp-st-set-minor-debug x interp-st))
+               ((interp-st-bind
+                 (equiv-contexts nil))
+                ((gl-interp-recursive-call err interp-st state)
+                 ;; replaces the top of stack with the bindings
+                 (gl-interp-bindinglist x-bindings interp-st state)))
+
+               ((when err)
+                (b* ((interp-st (interp-st-pop-minor-frame interp-st)))
+                  (mv err nil interp-st state)))
+               ((mv err val interp-st state)
+                (gl-interp-term-equivs body interp-st state))
+               (interp-st (interp-st-pop-minor-frame interp-st)))
+            (mv err val interp-st state))
+          :fncall 
+          (b* (((when (and** (eq x.fn 'if) (eql (len x.args) 3)))
+                (gl-interp-if/or (first x.args)
+                                 (second x.args)
+                                 (third x.args)
+                                 interp-st state))
+               ((when (and** (eq x.fn 'return-last) (eql (len x.args) 3)))
+                (gl-interp-return-last (first x.args)
+                                       (second x.args)
+                                       (third x.args)
+                                       interp-st state))
+               
+               (scratch (interp-st-scratch interp-st))
+               ((interp-st-bind
+                 (equiv-contexts nil))
+                ((gl-interp-recursive-call err interp-st state)
+                 ;; pushes the results from the args onto the scratch frame
+                 (gl-interp-arglist x.args interp-st state)))
+
+               ((when err)
+                ;; pop off any arguments that were added to scratch before the error
+                (b* ((interp-st (interp-st-pop-scratch (- (len (interp-st-scratch interp-st))
+                                                          (len scratch))
+                                                       interp-st)))
+                  (mv err nil interp-st state))))
+            (gl-interp-fncall x.fn (len x.args) interp-st state))))
+
+      (define gl-interp-arglist ((args pseudo-term-listp)
+                                 (interp-st interp-st-bfrs-ok)
+                                 state)
+        :measure (list (nfix (interp-st->reclimit interp-st))
+                       2020 (pseudo-term-list-binding-count args) 20)
+        :returns (mv err
+                     new-interp-st
+                     new-state)
+        (b* (((when (atom args)) (mv nil interp-st state))
+             ((gl-interp-recursive-call err arg1 interp-st state)
+              (gl-interp-term-equivs (car args) interp-st state))
+             ((when err) (mv err interp-st state))
+             (interp-st (interp-st-push-scratch arg1 interp-st)))
+          (gl-interp-arglist (cdr args) interp-st state)))
+
+      (define gl-interp-bindinglist ((bindings cmr::bindinglist-p)
+                                     (interp-st interp-st-bfrs-ok)
+                                     state)
+        :measure (list (nfix (interp-st->reclimit interp-st))
+                       2020
+                       (cmr::bindinglist-count bindings)
+                       20)
+        :returns (mv err
+                     new-interp-st
+                     new-state)
+        (b* (((when (atom bindings)) (mv nil interp-st state))
+             ((cmr::binding x1) (car bindings))
+             ((gl-interp-recursive-call err interp-st state)
+              (gl-interp-arglist x1.args interp-st state))
+             ((when err) (mv err interp-st state))
+             (argslen (len x1.args))
+             (args (interp-st-peek-scratch argslen interp-st))
+             (interp-st (interp-st-pop-scratch argslen interp-st))
+             (interp-st (interp-st-add-minor-bindings (pairlis$ x1.formals args) interp-st)))
+          (gl-interp-bindinglist (cdr bindings) interp-st state)))
+      
+      (define gl-interp-fncall ((fn pseudo-fnsym-p)
+                                (arity natp)
+                                (interp-st interp-st-bfrs-ok)
+                                state)
+        :measure (list (nfix (interp-st->reclimit interp-st))
+                       0 0 1)
+        :returns (mv err
+                     (ans gl-object-p)
+                     new-interp-st
+                     new-state)
+        (b* (((gl-function-mode fn-mode)
+              (gl-function-mode-fix!
+               (cdr (hons-assoc-equal fn (table-alist 'gl-fn-modes (w state))))))
+             (args (interp-st-peek-scratch arity interp-st))
+             (interp-st (interp-st-pop-scratch arity interp-st))
+             ((mv successp ans)
+              (fncall-try-concrete-eval fn args fn-mode.dont-concrete-exec state))
+             ((when successp)
+              (mv nil ans interp-st state))
+             (reclimit (interp-st->reclimit interp-st))
+             ((when (zp reclimit))
+              (gl-interp-error
+               :msg (gl-msg "The recursion limit ran out.")))
+             (interp-st (interp-st-pushlist-scratch args interp-st))
+             ((interp-st-bind
+               (reclimit (1- reclimit) reclimit))
+              ((gl-interp-recursive-call err successp ans interp-st state)
+               (gl-rewrite-fncall fn arity fn-mode.dont-rewrite interp-st state)))
+             ((when err)
+              (b* ((interp-st (interp-st-pop-scratch arity interp-st)))
+                (mv err nil interp-st state)))
+             ((when successp)
+              (b* ((interp-st (interp-st-pop-scratch arity interp-st)))
+                (mv nil ans interp-st state)))
+             (args (take arity (interp-st-scratch interp-st)))
+             ((mv successp ans interp-st state)
+              (gl-primitive-fncall fn args fn-mode.dont-primitive-exec interp-st state))
+             ((when successp)
+              (b* ((interp-st (interp-st-pop-scratch arity interp-st)))
+                (mv nil ans interp-st state)))
+             ((interp-st-bind
+               (reclimit (1- reclimit) reclimit))
+              ((mv err successp ans interp-st state)
+               (gl-interp-fn-definition fn args fn-mode.dont-expand-def interp-st state)))
+             ((when err)
+              (b* ((interp-st (interp-st-pop-scratch arity interp-st)))
+                (mv err nil interp-st state)))
+             ((when successp)
+              (b* ((interp-st (interp-st-pop-scratch arity interp-st)))
+                (mv nil ans interp-st state)))
+             (args (take arity (interp-st-scratch interp-st))))
+          (mv nil (g-apply fn args) interp-st state)))
+
+      (define gl-interp-fn-definition ((fn pseudo-fnsym-p)
+                                       (args gl-objectlist-p)
+                                       (dont)
+                                       (interp-st interp-st-bfrs-ok)
+                                       state)
+        :guard (interp-st-bfr-listp (gl-objectlist-bfrlist args))
+        :measure (list (nfix (interp-st->reclimit interp-st)) 20000 0 0)
+        :returns (mv err successp
+                     (ans gl-object-p)
+                     new-interp-st
+                     new-state)
+        (b* (((when dont)
+              (mv nil nil nil interp-st state))
+             ((mv ok body formals)
+              (acl2::fn-get-def fn state))
+             ((unless ok)
+              (mv nil nil nil interp-st state))
+             ((unless (eql (len formals) (len args)))
+              (gl-interp-error
+               :msg (gl-msg "Error interpreting a call of ~x0: it was given ~x1 arguments but has ~x2 formals."
+                            fn (len args) (len formals))
+               :nvals 2))
+             (interp-st (interp-st-push-frame (pairlis$ formals args) interp-st))
+             (interp-st (interp-st-set-debug fn interp-st))
+             ((mv err ans interp-st state)
+              (gl-interp-term-equivs body interp-st state))
+             (interp-st (interp-st-pop-frame interp-st)))
+          (mv err (not err) ans interp-st state)))
 
 
-  (define gl-interp-add-constraints-for-substs ((substs constraint-instancelist-p)
-                                                interp-st
+      (define gl-rewrite-fncall ((fn pseudo-fnsym-p)
+                                 (arity natp)
+                                 (dont)
+                                 (interp-st interp-st-bfrs-ok)
+                                 state)
+        ;; :guard (interp-st-bfr-listp (gl-objectlist-bfrlist args))
+        :measure (list (nfix (interp-st->reclimit interp-st)) 20000 0 0)
+        :returns (mv err successp
+                     (ans gl-object-p)
+                     new-interp-st
+                     new-state)
+        (b* (((when dont)
+              (mv nil nil nil interp-st state))
+             (rules (fn-rewrite-rules fn (glcp-config->rewrite-rule-table
+                                          (interp-st->config interp-st))
+                                      (w state)))
+             ((unless rules)
+              (mv nil nil nil interp-st state))
+             (reclimit (interp-st->reclimit interp-st))
+             ((when (zp reclimit))
+              (gl-interp-error
+               :msg (gl-msg "The recursion limit ran out.")
+               :nvals 2)))
+          (gl-rewrite-try-rules rules fn arity interp-st state)))
+
+      (define gl-rewrite-try-rules ((rules pseudo-rewrite-rule-listp)
+                                    (fn pseudo-fnsym-p)
+                                    (arity natp)
+                                    (interp-st interp-st-bfrs-ok)
+                                    state)
+        ;; :guard (interp-st-bfr-listp (gl-objectlist-bfrlist args))
+        :measure (list (nfix (interp-st->reclimit interp-st)) 10000 (len rules) 0)
+        :returns (mv err successp
+                     (ans gl-object-p)
+                     new-interp-st
+                     new-state)
+        (b* (((when (atom rules))
+              (mv nil nil nil interp-st state))
+             ((gl-interp-recursive-call err successp ans interp-st state)
+              (gl-rewrite-try-rule (car rules) fn arity interp-st state))
+             ((when (or err successp))
+              (mv err successp ans interp-st state)))
+          (gl-rewrite-try-rules (cdr rules) fn arity interp-st state)))
+
+      (define gl-rewrite-try-rule ((rule pseudo-rewrite-rule-p)
+                                   (fn pseudo-fnsym-p)
+                                   (arity natp)
+                                   (interp-st interp-st-bfrs-ok)
+                                   state)
+        ;; :guard (interp-st-bfr-listp (gl-objectlist-bfrlist args))
+        :measure (list (nfix (interp-st->reclimit interp-st)) 10000 0 0)
+        :returns (mv err successp
+                     (ans gl-object-p)
+                     new-interp-st
+                     new-state)
+        (b* (((acl2::rewrite-rule rule))
+             ((unless (and** (mbt (and* (symbolp rule.equiv)
+                                        (not (eq rule.equiv 'quote))
+                                        ;; (ensure-equiv-relationp rule.equiv (w state))
+                                        (not (eq rule.subclass 'acl2::meta))
+                                        (pseudo-termp rule.lhs)))
+                             (pseudo-term-case rule.lhs
+                               :fncall (and (eq rule.lhs.fn (pseudo-fnsym-fix fn))
+                                            (eql (len rule.lhs.args) (lnfix arity)))
+                               :otherwise nil)))
+              (gl-interp-error
+               :msg (gl-msg "Malformed rewrite rule: ~x0~%" rule)
+               :nvals 2))
+             ((unless (or (eq rule.equiv 'equal)
+                          ;; bozo check refinements
+                          (member rule.equiv (interp-st->equiv-contexts interp-st))))
+              (mv nil nil nil interp-st state))
+             (rule.lhs.args (pseudo-term-call->args rule.lhs))
+             ((mv unify-ok bindings) (glcp-unify-term/gobj-list-prefix rule.lhs.args
+                                                                       (interp-st-scratch interp-st)
+                                                                       nil))
+             ((unless unify-ok) (mv nil nil nil interp-st state))
+             ((unless (mbt (pseudo-term-listp rule.hyps)))
+              (gl-interp-error
+               :msg (gl-msg "Malformed rewrite rule: ~x0~%" rule)
+               :nvals 2))
+             (backchain-limit (interp-st->backchain-limit interp-st))
+             ((when (and** rule.hyps (eql 0 backchain-limit)))
+              (mv nil nil nil interp-st state))
+             (flags (interp-st->flags interp-st))
+             (hyps-flags  (!interp-flags->intro-synvars
+                           t
+                           (!interp-flags->intro-bvars
+                            nil
+                            (!interp-flags->simplify-logic nil flags))))
+             (interp-st (interp-st-push-frame bindings interp-st))
+             (interp-st (interp-st-set-debug rule interp-st))
+             ((interp-st-bind
+               (flags hyps-flags flags)
+               (equiv-contexts '(iff))
+               (backchain-limit (1- backchain-limit) backchain-limit))
+              ((gl-interp-recursive-call err successp interp-st state)
+               (gl-rewrite-relieve-hyps rule.hyps interp-st state)))
+
+             ((unless successp)
+              (b* ((interp-st (interp-st-pop-frame interp-st)))
+                (mv err nil nil interp-st state)))
+
+             (concl-flags (!interp-flags->intro-synvars t flags))
+             ((interp-st-bind
+               (flags concl-flags flags))
+              ((mv err val interp-st state)
+               (gl-interp-term-equivs rule.rhs interp-st state)))
+
+             (interp-st (interp-st-pop-frame interp-st)))
+
+          (mv err (not err) val interp-st state)))
+      
+      (define gl-rewrite-relieve-hyps ((hyps pseudo-term-listp)
+                                       (interp-st interp-st-bfrs-ok)
+                                       state)
+        :measure (list (nfix (interp-st->reclimit interp-st)) 9000
+                       (pseudo-term-list-binding-count hyps) 0)
+        :returns (mv err successp
+                     new-interp-st
+                     new-state)
+        (b* (((when (atom hyps))
+              (mv nil t interp-st state))
+             ((gl-interp-recursive-call err ok interp-st state)
+              (gl-rewrite-relieve-hyp (car hyps) interp-st state))
+             ((when (or err (not ok)))
+              (mv err ok interp-st state)))
+          (gl-rewrite-relieve-hyps (cdr hyps) interp-st state)))
+
+      (define gl-rewrite-relieve-hyp ((hyp pseudo-termp)
+                                      (interp-st interp-st-bfrs-ok)
+                                      state)
+        :measure (list (nfix (interp-st->reclimit interp-st)) 9000
+                       (pseudo-term-binding-count hyp) 0)
+        :returns (mv err successp
+                     new-interp-st
+                     new-state)
+        (b* (((mv synp-type untrans-form trans-term vars)
+              (gl-interp-match-synp hyp))
+             ((when synp-type)
+              (gl-rewrite-relieve-hyp-synp synp-type trans-term vars untrans-form interp-st state))
+             ((mv err test-bfr interp-st state)
+              (gl-interp-test hyp interp-st state)))
+          (mv err (eq test-bfr t) interp-st state)))
+
+      (define gl-interp-time$ ((timing-arg pseudo-termp)
+                               (x pseudo-termp)
+                               (interp-st interp-st-bfrs-ok)
+                               state)
+        :measure (list (nfix (interp-st->reclimit interp-st)) 2020
+                       (+ (pseudo-term-binding-count timing-arg)
+                          (pseudo-term-binding-count x))
+                       30)
+        :returns (mv err
+                     (ans gl-object-p)
+                     new-interp-st
+                     new-state)
+        (b* (((interp-st-bind
+               (equiv-contexts nil))
+              ((gl-interp-recursive-call err time$-arg interp-st state)
+               (gl-interp-term-equivs timing-arg interp-st state)))
+             ((when err)
+              (mv err nil interp-st state))
+             (time$-arg (gl-interp-time$-arg time$-arg x)))
+          (acl2::time$1 time$-arg
+                        (gl-interp-term-equivs x interp-st state))))
+      
+      (define gl-interp-return-last ((return-last-fnname pseudo-termp)
+                                     (first-arg pseudo-termp)
+                                     (last-arg pseudo-termp)
+                                     interp-st state)
+        :measure (list (nfix (interp-st->reclimit interp-st)) 2020
+                       (+ (pseudo-term-binding-count first-arg)
+                          (pseudo-term-binding-count last-arg))
+                       40)
+        :returns (mv err
+                     (ans gl-object-p)
+                     new-interp-st
+                     new-state)
+        (b* (((when (equal return-last-fnname ''time$1-raw))
+              (gl-interp-time$ first-arg last-arg interp-st state))
+             ((when (equal return-last-fnname ''(syntax-bind)))
+              (gl-interp-syntax-bind first-arg last-arg interp-st state)))
+          ;; Otherwise just evaluate the last-arg.
+          (gl-interp-term-equivs last-arg interp-st state)))
+      
+      
+
+      (define gl-interp-if/or ((test pseudo-termp)
+                               (then pseudo-termp)
+                               (else pseudo-termp)
+                               (interp-st interp-st-bfrs-ok)
+                               state)
+        :measure (list (nfix (interp-st->reclimit interp-st))
+                       2020
+                       (+ (pseudo-term-binding-count test)
+                          (pseudo-term-binding-count then)
+                          (pseudo-term-binding-count else))
+                       60)
+        :returns (mv err
+                     (ans gl-object-p)
+                     new-interp-st
+                     new-state)
+        (if (hons-equal test then)
+            (gl-interp-or test else interp-st state)
+          (gl-interp-if test then else interp-st state)))
+
+      
+      (define gl-interp-if ((test pseudo-termp)
+                            (then pseudo-termp)
+                            (else pseudo-termp)
+                            (interp-st interp-st-bfrs-ok)
+                            state)
+        :measure (list (nfix (interp-st->reclimit interp-st))
+                       2020
+                       (+ (pseudo-term-binding-count test)
+                          (pseudo-term-binding-count then)
+                          (pseudo-term-binding-count else))
+                       40)
+        :returns (mv err
+                     (ans gl-object-p)
+                     new-interp-st
+                     new-state)
+        ;; Tricky because we have to keep the test/thenval on the stack while we
+        ;; run the then/else branches, because we might simplify the logicman while
+        ;; running them.
+        (b* (((gl-interp-recursive-call err testbfr interp-st state)
+              (gl-interp-test test interp-st state))
+             ((when err) (mv err nil interp-st state))
+             (interp-st (interp-st-push-bool-scratch testbfr interp-st))
+             ((gl-interp-recursive-call err then-unreachable thenval interp-st state)
+              ;; pushes val onto scratch if not unreachable
+              (gl-maybe-interp testbfr then interp-st state))
+             ((when err)
+              (b* ((interp-st (interp-st-pop-bool-scratch 1 interp-st)))
+                (mv err nil interp-st state)))
+             (interp-st (interp-st-push-scratch thenval interp-st))
+             ;; note: testbool may have changed if we simplified the logicman
+             (testbfr (first (interp-st-bool-scratch interp-st)))
+             ((gl-interp-recursive-call err else-unreachable elseval interp-st state)
+              ;; pushes val onto scratch if not unreachable
+              (gl-maybe-interp (interp-st-bfr-not testbfr) else interp-st state))
+             ((when err)
+              (b* ((interp-st (interp-st-pop-scratch 1 interp-st))
+                   (interp-st (interp-st-pop-bool-scratch 1 interp-st)))
+                (mv err nil interp-st state)))
+             (thenval (first (interp-st-scratch interp-st)))
+             (testbfr (first (interp-st-bool-scratch interp-st)))
+             (interp-st (interp-st-pop-scratch 1 interp-st))
+             (interp-st (interp-st-pop-bool-scratch 1 interp-st))
+             ((when then-unreachable)
+              (if else-unreachable
+                  (mv :unreachable nil interp-st state)
+                (mv nil elseval interp-st state)))
+             ((when else-unreachable)
+              (mv nil thenval interp-st state)))
+          (gl-interp-merge-branches testbfr thenval elseval interp-st state)))
+
+      (define gl-interp-or ((test pseudo-termp)
+                            (else pseudo-termp)
+                            (interp-st interp-st-bfrs-ok)
+                            state)
+        :measure (list (nfix (interp-st->reclimit interp-st))
+                       2020
+                       (+ (pseudo-term-binding-count test)
+                          (pseudo-term-binding-count else))
+                       40)
+        :returns (mv err
+                     (ans gl-object-p)
+                     new-interp-st
+                     new-state)
+        (b* ((equiv-contexts (interp-st->equiv-contexts interp-st))
+             (or-test-equiv-contexts (gl-interp-or-test-equiv-contexts equiv-contexts))
+             ((interp-st-bind
+               (equiv-contexts or-test-equiv-contexts equiv-contexts))
+              ((gl-interp-recursive-call err testval interp-st state)
+               (gl-interp-term-equivs test interp-st state)))
+             ((when err) (mv err nil interp-st state))
+             ((gl-interp-recursive-call err testbfr interp-st state)
+              (gl-interp-simplify-if-test testval interp-st state))
+             ((when err) (mv err nil interp-st state))
+             (interp-st (interp-st-push-scratch testval interp-st))
+             (interp-st (interp-st-push-bool-scratch testbfr interp-st))
+             ((gl-interp-recursive-call err else-unreachable elseval interp-st state)
+              ;; pushes val onto scratch if not unreachable
+              (gl-maybe-interp (interp-st-bfr-not testbfr) else interp-st state))
+             (testval (first (interp-st-scratch interp-st)))
+             (testbfr (first (interp-st-bool-scratch interp-st)))
+             (interp-st (interp-st-pop-scratch 1 interp-st))
+             (interp-st (interp-st-pop-bool-scratch 1 interp-st))
+             ((when err)
+              (mv err nil interp-st state))
+             ((when else-unreachable)
+              (mv nil testval interp-st state)))
+          (gl-interp-merge-branches testbfr testval elseval interp-st state)))
+
+
+      (define gl-maybe-interp ((test interp-st-bfr-p)
+                               (x pseudo-termp)
+                               (interp-st interp-st-bfrs-ok)
+                               state)
+        :measure (list (nfix (interp-st->reclimit interp-st))
+                       2020
+                       (pseudo-term-binding-count x)
+                       60)
+        :returns (mv err
+                     unreachable
+                     (ans gl-object-p)
+                     new-interp-st
+                     new-state)
+        (b* (((mv contra checkpoint interp-st)
+              (interp-st-pathcond-assume test interp-st))
+             ((when contra)
+              (mv nil t nil interp-st state))
+             ((mv err ans interp-st state)
+              (gl-interp-term-equivs x interp-st state))
+             (interp-st (stobj-let ((logicman (interp-st->logicman interp-st))
+                                    (pathcond (interp-st->pathcond interp-st)))
+                                   (pathcond)
+                                   (pathcond-rewind checkpoint (lbfr-mode logicman) pathcond)
+                                   interp-st))
+             ((when (eq err :unreachable))
+              (mv nil t nil interp-st state)))
+          (mv err nil ans interp-st state)))
+
+      (define gl-interp-maybe-simplify-if-test ((test interp-st-bfr-p)
+                                                (xobj gl-object-p)
+                                                (interp-st interp-st-bfrs-ok)
                                                 state)
-    :guard (gl-object-case x :g-apply)
-    :measure (list (nfix (interp-st->reclimit interp-st))
-                   2000
-                   (gl-object-count x)
-                   10)
-    :returns (mv err
-                 new-interp-st
-                 new-state)
-    (b* (((when (atom substs)) (mv nil interp-st state))
-         ((constraint-instance sub1) (car substs))
-         (thm-body (meta-extract-formula sub1.thmname state))
-         ((unless (pseudo-termp thm-body))
-          (gl-interp-add-constraints-for-substs (cdr substs) interp-st state))
-         (interp-st (interp-st-push-frame sub1.subst interp-st))
-         ((mv err bfr interp-st state)
-          (gl-interp-test thm-body interp-st state))
-         (interp-st (interp-st-pop-frame interp-st))
-         ((mv contra interp-st) (stobj-let ((constraint-pathcond (interp-st->constraint interp-st))
-                                            (logicman (interp-st->logicman interp-st)))
-                                           (contra pathcond)
-                                           (logicman-pathcond-assume bfr constraint-pathcond)
-                                           (mv contra interp-st)))
-         ((when contra)
-          (mv (gl-msg "A contradiction has been noted in the constraints.  ~
-                       This is likely due to a bug in GL or an unsound fact ~
-                       stored in ACL2 (e.g., via TTAG,skip-proofs, defaxiom, ~
-                       or soundness bug).")
-              interp-st state)))
-      (gl-interp-add-constraints-for-substs (cdr substs) interp-st state)))
-         
+        :guard (interp-st-bfr-listp (gl-object-bfrlist xobj))
+        :measure (list (nfix (interp-st->reclimit interp-st))
+                       2000
+                       (gl-object-count xobj)
+                       60)
+        :returns (mv err
+                     unreachable
+                     xbfr
+                     new-interp-st
+                     new-state)
+        (b* (((mv contra checkpoint interp-st)
+              (interp-st-pathcond-assume test interp-st))
+             ((when contra)
+              (mv nil t nil interp-st state))
+             ((mv err ans interp-st state)
+              (gl-interp-simplify-if-test xobj interp-st state))
+             (interp-st (stobj-let ((logicman (interp-st->logicman interp-st))
+                                    (pathcond (interp-st->pathcond interp-st)))
+                                   (pathcond)
+                                   (pathcond-rewind checkpoint (lbfr-mode logicman) pathcond)
+                                   interp-st))
+             ((when (eq err :unreachable))
+              (mv nil t nil interp-st state)))
+          (mv err nil ans interp-st state)))
 
-  gl-rewrite-relieve-hyps
-    gl-interp-merge-branches)
-             
+      (define gl-interp-simplify-if-test ((xobj gl-object-p)
+                                          (interp-st interp-st-bfrs-ok)
+                                          state)
+        :guard (interp-st-bfr-listp (gl-object-bfrlist xobj))
+        :returns (mv err
+                     xbfr
+                     new-interp-st
+                     new-state)
+        :measure (list (nfix (interp-st->reclimit interp-st))
+                       2000
+                       (gl-object-count xobj)
+                       40)
+        (gl-object-case xobj
+          :g-concrete (mv nil (bool-fix xobj.val) interp-st state)
+          :g-boolean (mv nil xobj.bool interp-st state)
+          :g-integer (mv nil t interp-st state)
+          :g-cons (mv nil t interp-st state)
+          :g-var (stobj-let ((bvar-db (interp-st->bvar-db interp-st))
+                             (logicman (interp-st->logicman interp-st)))
+                            (bfr bvar-db)
+                            (b* (((mv bvar bvar-db) (add-term-bvar-unique xobj bvar-db))
+                                 (bvar-db (maybe-add-equiv-term xobj bvar bvar-db state))
+                                 (bfr (bfr-var bvar)))
+                              (mv bfr bvar-db))
+                            (mv nil bfr interp-st state))
+          :g-ite (b* (((gl-interp-recursive-call err test-bfr interp-st state)
+                       (gl-interp-simplify-if-test xobj.test interp-st state))
+                      ((when err)
+                       (mv err nil interp-st state))
+                      (interp-st (interp-st-push-bool-scratch test-bfr interp-st))
+                      ((gl-interp-recursive-call err then-unreachable then-bfr interp-st state)
+                       (gl-interp-maybe-simplify-if-test test-bfr xobj.then interp-st state))
+                      ((when err)
+                       (b* ((interp-st (interp-st-pop-bool-scratch 1 interp-st)))
+                         (mv err nil interp-st state)))
+                      (test-bfr (car (interp-st-bool-scratch interp-st)))
+                      (interp-st (interp-st-push-bool-scratch then-bfr interp-st))
+                      ((mv err else-unreachable else-bfr interp-st state)
+                       (gl-interp-maybe-simplify-if-test test-bfr xobj.else interp-st state))
+                      ((when err)
+                       (b* ((interp-st (interp-st-pop-bool-scratch 2 interp-st)))
+                         (mv err nil interp-st state)))
+                      (then-bfr (car (interp-st-bool-scratch interp-st)))
+                      (test-bfr (cadr (interp-st-bool-scratch interp-st)))
+                      ((when then-unreachable)
+                       (if else-unreachable
+                           (mv :unreachable nil interp-st state)
+                         (mv nil else-bfr interp-st state)))
+                      ((when else-unreachable)
+                       (mv nil then-bfr interp-st state))
+                      ((mv ite interp-st) (stobj-let ((logicman (interp-st->logicman interp-st)))
+                                                     (ite logicman)
+                                                     (bfr-ite test-bfr then-bfr else-bfr)
+                                                     (mv ite interp-st))))
+                   (mv nil ite interp-st state))
+          :g-apply (gl-interp-simplify-if-test-fncall xobj interp-st state)))
+
+      (define gl-interp-simplify-if-test-fncall ((xobj gl-object-p)
+                                                 (interp-st interp-st-bfrs-ok)
+                                                 state)
+        :guard (and (gl-object-case xobj :g-apply)
+                    (interp-st-bfr-listp (gl-object-bfrlist xobj)))
+
+        :measure (list (nfix (interp-st->reclimit interp-st))
+                       2000
+                       (gl-object-count xobj)
+                       20)
+        :returns (mv err
+                     xbfr
+                     new-interp-st
+                     new-state)
+        (b* (((mv not-matched neg-arg)
+              (gl-apply-match-not xobj))
+             ((when not-matched)
+              (b* (((mv err bfr interp-st state)
+                    (gl-interp-simplify-if-test neg-arg interp-st state))
+                   ((when err)
+                    (mv err nil interp-st state)))
+                (mv nil (interp-st-bfr-not bfr) interp-st state)))
+             ((g-apply xobj))
+             ((gl-function-mode fn-mode)
+              (gl-function-mode-fix!
+               (cdr (hons-assoc-equal xobj.fn (table-alist 'gl-fn-modes (w state))))))
+
+             ;; BOZO support gl-interp-force-check.
+
+             ;; We rewrite this fncall again because it presumably might not have
+             ;; been done in IFF context before.  E.g.
+             ;; (let ((a (foo x)))
+             ;;   (if a y z))
+             ;; Note we wouldn't do this fully "right" even if we had perfect
+             ;; knowledge of congruences because our test term might be bound to a
+             ;; variable that is used in both Boolean and non-Boolean contexts.
+             (reclimit (interp-st->reclimit interp-st))
+             ((when (zp reclimit))
+              (gl-interp-error
+               :msg (gl-msg "The recursion limit ran out.")))
+             ((interp-st-bind
+               (reclimit (1- reclimit) reclimit)
+               (equiv-contexts '(iff)))
+              ((gl-interp-recursive-call err successp ans interp-st state)
+               (gl-rewrite-fncall xobj.fn xobj.args fn-mode.dont-rewrite-under-if-test interp-st state)))
+             ((when err)
+              (mv err nil interp-st state))
+             ((when successp)
+              (b* (((interp-st-bind
+                     (reclimit (1- reclimit) reclimit))
+                    ((mv err ans interp-st state)
+                     (gl-interp-simplify-if-test ans interp-st state))))
+                (mv err ans interp-st state)))
+
+             (look (stobj-let ((bvar-db (interp-st->bvar-db interp-st)))
+                              (look)
+                              (get-term->bvar xobj bvar-db)
+                              look))
+             ((when look)
+              (b* ((bfr (stobj-let ((logicman (interp-st->logicman interp-st)))
+                                   (bfr)
+                                   (bfr-var look)
+                                   bfr)))
+                (mv nil bfr interp-st state)))
+
+             ((unless (interp-flags->intro-bvars (interp-st->flags interp-st)))
+              ;; Note: we only return intro-bvars-fail when this flag is set to
+              ;; false, which it is not at the top level.  So when we set the flag
+              ;; to true (as we do in relieve-hyp and add-bvar-constraint-substs,
+              ;; e.g.) we check for this error specifically and catch it.
+              ;; Otherwise we expect callers not to set intro-bvars to nil and then
+              ;; they won't have to deal with this error specially.
+              (mv :intro-bvars-fail nil interp-st state))
+
+             ((unless (gl-object-symbolic-boolean-free xobj))
+              (gl-interp-error
+               :msg (gl-msg "An object used as an IF test was not reduced to ~
+                             either a term-like object or a symbolic Boolean, ~
+                             i.e. it had both function calls and symbolic ~
+                             Boolean parts.  This isn't currently allowed.  ~
+                             The state global variable (~x0 ~x1) holds the object."
+                            '@ 'gl-interp-error-debug-obj)
+               :debug-obj xobj))
+
+             ((mv bfr interp-st)
+              (stobj-let ((bvar-db (interp-st->bvar-db interp-st))
+                          (logicman (interp-st->logicman interp-st)))
+                         (var bvar-db)
+                         (b* ((bvar (next-bvar bvar-db))
+                              (bvar-db (add-term-bvar xobj bvar-db))
+                              (bvar-db (maybe-add-equiv-term xobj bvar bvar-db state))
+                              (bfr (bfr-var bvar)))
+                           (mv bfr bvar-db))
+                         (mv var interp-st)))
+
+             ((mv err interp-st state)
+              (gl-interp-add-constraints xobj interp-st state))
+
+             ((when err)
+              (mv err nil interp-st state)))
+          (mv nil bfr interp-st state)))
+
+
+      (define gl-interp-add-constraints ((xobj gl-object-p)
+                                         (interp-st interp-st-bfrs-ok)
+                                         state)
+        :guard (and (gl-object-case xobj :g-apply)
+                    (interp-st-bfr-listp (gl-object-bfrlist xobj)))
+        :measure (list (nfix (interp-st->reclimit interp-st))
+                       2000
+                       (gl-object-count xobj)
+                       15)
+        :returns (mv err
+                     new-interp-st
+                     new-state)
+        (b* ((constraint-db (interp-st->constraint-db interp-st))
+             ((mv constraint-substs constraint-db)
+              (gbc-process-new-lit xobj constraint-db state))
+             (interp-st (update-interp-st->constraint-db constraint-db interp-st))
+             ((unless constraint-substs)
+              (mv nil interp-st state))
+             ;; Disable the pathcond so that constraint thms are simulated in an empty (universal) context.
+             ((mv pathcond-enabledp interp-st) (stobj-let ((pathcond (interp-st->pathcond interp-st)))
+                                                          (enabledp pathcond)
+                                                          (b* ((enabledp (pathcond-enabledp pathcond))
+                                                               (pathcond (update-pathcond-enabledp nil pathcond)))
+                                                            (mv enabledp pathcond))
+                                                          (mv enabledp interp-st)))
+             (reclimit (interp-st->reclimit interp-st))
+             ((when (zp reclimit))
+              (gl-interp-error :msg (gl-msg "The recursion limit ran out.") :nvals 0))
+             (interp-st (update-interp-st->constraint-inst-stack
+                         (append constraint-substs (interp-st->constraint-inst-stack interp-st))
+                         interp-st))
+             ((interp-st-bind
+               (reclimit (1- reclimit) reclimit))
+              ((mv err interp-st state)
+               (gl-interp-add-constraints-for-substs (len constraint-substs) interp-st state)))
+             (interp-st (stobj-let ((pathcond (interp-st->pathcond interp-st)))
+                                   (pathcond)
+                                   (update-pathcond-enabledp pathcond-enabledp pathcond)
+                                   interp-st)))
+          (mv err interp-st state)))
+      
+
+
+      (define gl-interp-add-constraints-for-substs ((n natp)
+                                                    (interp-st interp-st-bfrs-ok)
+                                                    state)
+        :guard (<= n (len (interp-st->constraint-inst-stack interp-st)))
+        :measure (list (nfix (interp-st->reclimit interp-st))
+                       10000
+                       (nfix n)
+                       10)
+        :returns (mv err
+                     new-interp-st
+                     new-state)
+        (b* (((when (zp n)) (mv nil interp-st state))
+             ((constraint-instance sub1) (car (interp-st->constraint-inst-stack interp-st)))
+             (interp-st (update-interp-st->constraint-inst-stack
+                         (cdr (interp-st->constraint-inst-stack interp-st))
+                         interp-st))
+             (thm-body (meta-extract-formula sub1.thmname state))
+             ((unless (pseudo-termp thm-body))
+              (gl-interp-add-constraints-for-substs (1- n) interp-st state))
+             (interp-st (interp-st-push-frame sub1.subst interp-st))
+             ((gl-interp-recursive-call err bfr interp-st state)
+              (gl-interp-test thm-body interp-st state))
+             (interp-st (interp-st-pop-frame interp-st))
+             ((when err)
+              (mv err interp-st state))
+             ((mv contra interp-st) (stobj-let ((constraint-pathcond (interp-st->constraint interp-st))
+                                                (logicman (interp-st->logicman interp-st)))
+                                               (contra constraint-pathcond)
+                                               (logicman-pathcond-assume bfr constraint-pathcond)
+                                               (mv contra interp-st)))
+             ((when contra)
+              (gl-interp-error
+               :msg (gl-msg "A contradiction has been noted in the ~
+                             constraints.  This is likely due to a bug in GL ~
+                             or an unsound fact stored in ACL2 (e.g., via ~
+                             TTAG, skip-proofs, defaxiom, or soundness bug). ~
+                             The constraint instance that led to the ~
+                             contradiction is stored in the state global (~x0 ~
+                             ~x1), but note that a previous constraint ~
+                             instance might have caused the unsoundness."
+                            '@ 'gl-interp-error-debug-obj)
+               :debug-obj sub1
+               :nvals 0)))
+          (gl-interp-add-constraints-for-substs (1- n) interp-st state)))
+      
+
+      (define gl-interp-merge-branches ((testbfr interp-st-bfr-p)
+                                        (thenval gl-object-p)
+                                        (elseval gl-object-p)
+                                        (interp-st interp-st-bfrs-ok)
+                                        state)
+        :guard (and (interp-st-bfr-listp (gl-object-bfrlist thenval))
+                    (interp-st-bfr-listp (gl-object-bfrlist elseval)))
+        :measure (list (nfix (interp-st->reclimit interp-st))
+                       2000
+                       (+ (gl-object-count thenval)
+                          (gl-object-count elseval))
+                       40)
+        :returns (mv err
+                     (ans gl-object-p)
+                     new-interp-st
+                     new-state)
+        (b* ((thenval (gl-object-fix thenval))
+             (elseval (gl-object-fix elseval))
+             ((when (eq testbfr t)) (mv nil thenval interp-st state))
+             ((when (eq testbfr nil)) (mv nil elseval interp-st state))
+             ((when (hons-equal thenval elseval)) (mv nil thenval interp-st state)))
+          (gl-interp-merge-branches-rewrite testbfr thenval elseval nil interp-st state)))
+
+      (define gl-interp-merge-branches-rewrite ((testbfr interp-st-bfr-p)
+                                                (thenval gl-object-p)
+                                                (elseval gl-object-p)
+                                                switchedp
+                                                (interp-st interp-st-bfrs-ok)
+                                                state)
+        :guard (and (interp-st-bfr-listp (gl-object-bfrlist thenval))
+                    (interp-st-bfr-listp (gl-object-bfrlist elseval)))
+        :measure (list (nfix (interp-st->reclimit interp-st))
+                       2000
+                       (+ (gl-object-count thenval)
+                          (gl-object-count elseval))
+                       (if switchedp 20 30))
+        :returns (mv err
+                     (ans gl-object-p)
+                     new-interp-st
+                     new-state)
+        (b* ((thenval (gl-object-fix thenval))
+             (elseval (gl-object-fix elseval))
+             (fn (gl-fncall-object->fn thenval))
+             (rules (and** fn (fn-branch-merge-rules fn 
+                                                   (glcp-config->branch-merge-rules
+                                                    (interp-st->config interp-st))
+                                                   (w state))))
+             ((unless rules)
+              ;; Note: we try to apply if-merge rules based on the leading function
+              ;; symbol of the then or else objects.  We try then first
+              ;; (switchedp=nil), then else (switchedp=t), and if both fail we move
+              ;; on to merge-branches-subterms.
+              (if switchedp
+                  (gl-interp-merge-branch-subterms
+                   (interp-st-bfr-not testbfr)
+                   elseval thenval interp-st state)
+                (gl-interp-merge-branches-rewrite
+                 (interp-st-bfr-not testbfr)
+                 elseval thenval t interp-st state)))
+
+             (reclimit (interp-st->reclimit interp-st))
+             ((when (zp reclimit))
+              (gl-interp-error :msg (gl-msg "The recursion limit ran out.")))
+             ((interp-st-bind
+               (reclimit (1- reclimit) reclimit))
+              ((mv err successp ans interp-st state)
+               (gl-rewrite-try-rules rules 'if (list (g-boolean testbfr) thenval elseval) interp-st state)))
+             ((when err) (mv err nil interp-st state))
+             ((when successp)
+              (mv nil ans interp-st state)))
+          (if switchedp
+              (gl-interp-merge-branch-subterms
+               (interp-st-bfr-not testbfr)
+               elseval thenval interp-st state)
+            (gl-interp-merge-branches-rewrite
+             (interp-st-bfr-not testbfr)
+             elseval thenval t interp-st state))))
+
+      (define gl-interp-merge-branch-subterms ((testbfr interp-st-bfr-p)
+                                               (thenval gl-object-p)
+                                               (elseval gl-object-p)
+                                               (interp-st interp-st-bfrs-ok)
+                                               state)
+        :guard (and (interp-st-bfr-listp (gl-object-bfrlist thenval))
+                    (interp-st-bfr-listp (gl-object-bfrlist elseval)))
+        :measure (list (nfix (interp-st->reclimit interp-st))
+                       2000
+                       (+ (gl-object-count thenval)
+                          (gl-object-count elseval))
+                       10)
+        :returns (mv err
+                     (ans gl-object-p)
+                     new-interp-st
+                     new-state)
+        (b* (((mv thenfn thenargs) (gl-object-recognize-merge-fncall thenval))
+             ((mv elsefn elseargs) (gl-object-recognize-merge-fncall elseval))
+             ((unless (and** thenfn
+                             (eq thenfn elsefn)
+                             (eql (len thenargs) (len elseargs))))
+              (stobj-let ((logicman (interp-st->logicman interp-st)))
+                         (obj logicman)
+                         (gl-object-basic-merge testbfr thenval elseval)
+                         (mv nil obj interp-st state)))
+             (scratch (interp-st-scratch interp-st))
+             (thenval-stack (interp-st->thenval-stack interp-st))
+             (elseval-stack (interp-st->elseval-stack interp-st))
+             (interp-st (update-interp-st->thenval-stack (append thenargs thenval-stack) interp-st))
+             (interp-st (update-interp-st->elseval-stack (append elseargs elseval-stack) interp-st))
+             (interp-st (interp-st-push-bool-scratch testbfr interp-st))
+             ;; pops args off thenval/elseval-stack, pushes onto scratch
+             ((gl-interp-recursive-call err interp-st state)
+              (gl-interp-merge-branch-args (len thenargs) interp-st state))
+             (interp-st (interp-st-pop-bool-scratch 1 interp-st))
+             ((when err)
+              ;; pop off any args pushed on before error
+              (b* ((interp-st (interp-st-pop-scratch (- (len (interp-st-scratch interp-st))
+                                                        (len scratch))
+                                                     interp-st))
+                   ;; (new-thenval-stack (interp-st->thenval-stack interp-st))
+                   ;; (interp-st (update-interp-st->thenval-stack
+                   ;;             (nthcdr (- (len new-thenval-stack)
+                   ;;                        (len thenval-stack))
+                   ;;                     new-thenval-stack)
+                   ;;             interp-st))
+                   ;; (new-elseval-stack (interp-st->elseval-stack interp-st))
+                   ;; (interp-st (update-interp-st->elseval-stack
+                   ;;             (nthcdr (- (len new-elseval-stack)
+                   ;;                        (len elseval-stack))
+                   ;;                     new-elseval-stack)
+                   ;;             interp-st))
+                   )
+                (mv err nil interp-st state))))
+          (gl-interp-fncall thenfn (len thenargs) interp-st state)))
+
+      (define gl-interp-merge-branch-args (;; (testbfr interp-st-bfr-p)
+                                           (n natp)
+                                           ;; (thenargs gl-objectlist-p)
+                                           ;; (elseargs gl-objectlist-p)
+                                           (interp-st interp-st-bfrs-ok)
+                                           state)
+        ;; :guard (and (eql (len thenargs) (len elseargs))
+        ;;             (interp-st-bfr-listp (gl-objectlist-bfrlist thenargs))
+        ;;             (interp-st-bfr-listp (gl-objectlist-bfrlist elseargs)))
+        :measure (list (nfix (interp-st->reclimit interp-st))
+                       1000
+                       (nfix n)
+                       5)
+        :returns (mv err
+                     new-interp-st
+                     new-state)
+        (b* (((when (zp n))
+              (mv nil interp-st state))
+             (thenstack (interp-st->thenval-stack interp-st))
+             (thenval (car thenstack))
+             (interp-st (update-interp-st->thenval-stack (cdr thenstack) interp-st))
+             (elsestack (interp-st->elseval-stack interp-st))
+             (elseval (car elsestack))
+             (interp-st (update-interp-st->elseval-stack (cdr elsestack) interp-st))
+             ;; BOZO sad:
+             (reclimit (interp-st->reclimit interp-st))
+             ((when (zp reclimit))
+              (gl-interp-error :msg (gl-msg "The recursion limit ran out.") :nvals 0))
+             ((interp-st-bind
+               (reclimit (1- reclimit) reclimit))
+              ((mv err ans interp-st state)
+               (gl-interp-merge-branches (car (interp-st-bool-scratch interp-st))
+                                         thenval elseval interp-st state)))
+             ((when err)
+              (b* ((interp-st (update-interp-st->thenval-stack
+                               (nthcdr (1- n) (interp-st->thenval-stack interp-st))
+                               interp-st))
+                   (interp-st (update-interp-st->elseval-stack
+                               (nthcdr (1- n) (interp-st->elseval-stack interp-st))
+                               interp-st)))
+                (mv err interp-st state)))
+             (interp-st (interp-st-push-scratch ans interp-st)))
+          (gl-interp-merge-branch-args (1- n) interp-st state))))))
+
+
+
+
+
+(local
+ (defthm major-stack-bfrlist-of-stack$a-push-scratch
+   (acl2::set-equiv (major-stack-bfrlist (stack$a-push-scratch obj stack))
+              (append (gl-object-bfrlist obj)
+                      (major-stack-bfrlist stack)))
+   :hints(("Goal" :in-theory (enable major-stack-bfrlist
+                                     major-frame-bfrlist
+                                     minor-stack-bfrlist
+                                     minor-frame-bfrlist
+                                     stack$a-push-scratch)))))
+
+(local
+ (defthm major-stack-bfrlist-of-stack$a-push-bool-scratch
+   (acl2::set-equiv (major-stack-bfrlist (stack$a-push-bool-scratch obj stack))
+                    (cons obj
+                          (major-stack-bfrlist stack)))
+   :hints(("Goal" :in-theory (enable stack$a-push-bool-scratch
+                                     major-stack-bfrlist
+                                     major-frame-bfrlist
+                                     minor-frame-bfrlist
+                                     minor-stack-bfrlist
+                                     acl2::set-unequal-witness-rw)
+           :do-not-induct t
+           :expand ((major-stack-bfrlist stack)
+                    (major-frame-bfrlist (car stack))
+                    (minor-stack-bfrlist (major-frame->minor-stack (car stack)))
+                    (minor-frame-bfrlist (car (major-frame->minor-stack (car stack)))))))))
+
+(local (defthm bfr-listp-of-gl-objectlist-bfrlist-cdr
+         (implies (bfr-listp (gl-objectlist-bfrlist x))
+                  (bfr-listp (gl-objectlist-bfrlist (cdr x))))
+         :hints(("Goal" :in-theory (enable gl-objectlist-bfrlist)))))
+
+(local (defthm bfr-listp-of-gl-objectlist-bfrlist-nthcdr
+         (implies (bfr-listp (gl-objectlist-bfrlist x))
+                  (bfr-listp (gl-objectlist-bfrlist (nthcdr n x))))
+         :hints(("Goal" :in-theory (enable nthcdr)))))
+
+(local (defthm bfr-listp-of-gl-object-bfrlist-car
+         (implies (bfr-listp (gl-objectlist-bfrlist x))
+                  (bfr-listp (gl-object-bfrlist (car x))))
+         :hints(("Goal" :expand ((gl-objectlist-bfrlist x))
+                 :in-theory (enable default-car)))))
+
+(local (defthm bfr-p-car-of-bfr-list
+         (implies (bfr-listp x)
+                  (bfr-p (car x)))
+         :hints(("Goal" :in-theory (enable default-car bfr-listp)))))
+
+(local (defthm bfr-listp-of-bool-scratch-when-stack-ok
+         (implies (bfr-listp (major-stack-bfrlist stack))
+                  (bfr-listp (stack$a-bool-scratch stack)))
+         :hints(("Goal" :in-theory (enable stack$a-bool-scratch)
+                 :expand ((major-stack-bfrlist stack)
+                          (major-frame-bfrlist (car stack))
+                          (minor-stack-bfrlist (major-frame->minor-stack (car stack)))
+                          (minor-frame-bfrlist (car (major-frame->minor-stack (car stack)))))
+                 :do-not-induct t))))
+
+(local (defthm gl-objectlist-bfrlist-of-append
+         (equal (gl-objectlist-bfrlist (append x y))
+                (append (gl-objectlist-bfrlist x)
+                        (gl-objectlist-bfrlist y)))
+         :hints(("Goal" :in-theory (enable gl-objectlist-bfrlist)))))
+
+(local (in-theory (disable bfrlist-okp-of-gl-objectlist-bfrlist
+                           bfr-listp-of-gl-object-bfrlist)))
+
+(progn
+  (with-output
+    :off (event prove)
+    (std::defret-mutual-generate interp-st-bfrs-ok-of-<fn>
+      :formal-hyps (((interp-st-bfr-p x)           (interp-st-bfr-p x))
+                    ((gl-object-p x)               (interp-st-bfr-listp (gl-object-bfrlist x)))
+                    ((gl-objectlist-p x)           (interp-st-bfr-listp (gl-objectlist-bfrlist x)))
+                    (interp-st                     (interp-st-bfrs-ok interp-st))
+                    ((constraint-instancelist-p x) (interp-st-bfr-listp (constraint-instancelist-bfrlist x))))
+      :return-concls ((xbfr                        (interp-st-bfr-p xbfr :interp-st new-interp-st))
+                      ((gl-object-p x)             (interp-st-bfr-listp (gl-object-bfrlist x) :interp-st new-interp-st))
+                      (new-interp-st               (interp-st-bfrs-ok new-interp-st)))
+      :rules ((t (:add-keyword :hints ('(:expand (<call>) :do-not-induct t))))))))
+
+                
+         
+         
         
          
     
